Move operations and aliasing theorem to separate file.

pointers.v
@@ -38,52 +38,8 @@ Section pointer_operations.
     | Ptr a => type_check (Γ,Γm) a
     end.
   Inductive is_NULL : ptr Ti → Prop := mk_is_NULL τ : is_NULL (NULL τ).
-
   Definition ptr_alive (Γm : memenv Ti) (p : ptr Ti) : Prop :=
     match p with NULL _ => True | Ptr a => index_alive Γm (addr_index a) end.
-  Definition ptr_compare_ok (Γm : memenv Ti) (c : compop) (p1 p2 : ptr Ti) : Prop :=
-    match p1, p2 with
-    | Ptr a1, Ptr a2 => addr_minus_ok Γm a1 a2
-    | NULL _, Ptr a2 =>
-       match c with EqOp => index_alive Γm (addr_index a2) | _ => False end
-    | Ptr a1, NULL _ =>
-       match c with EqOp => index_alive Γm (addr_index a1) | _ => False end
-    | NULL _, NULL _ => True
-    end.
-  Definition ptr_compare (Γ : env Ti) (c : compop) (p1 p2 : ptr Ti) : bool :=
-    match p1, p2 with
-    | Ptr a1, Ptr a2 => Z_comp c (addr_minus Γ a1 a2) 0
-    | NULL _, Ptr a2 => false (* only allowed for EqOp *)
-    | Ptr a1, NULL _ => false (* only allowed for EqOp *)
-    | NULL _, NULL _ => match c with EqOp | LeOp => true | LtOp => false end
-    end.
-  Definition ptr_plus_ok (Γ : env Ti) (Γm : memenv Ti) (j : Z) (p : ptr Ti) :=
-    match p with NULL _ => j = 0 | Ptr a => addr_plus_ok Γ Γm j a end.
-  Global Arguments ptr_plus_ok _ _ _ !_ /.
-  Definition ptr_plus (Γ : env Ti) (j : Z) (p : ptr Ti) : ptr Ti :=
-    match p with NULL τ => NULL τ | Ptr a => Ptr (addr_plus Γ j a) end.
-  Global Arguments ptr_plus _ _ !_ /.
-  Definition ptr_minus_ok (Γm : memenv Ti) (p1 p2 : ptr Ti) : Prop :=
-    match p1, p2 with
-    | NULL _, NULL _ => True
-    | Ptr a1, Ptr a2 => addr_minus_ok Γm a1 a2
-    | _, _ => False
-    end.
-  Global Arguments ptr_minus_ok _ !_ !_ /.
-  Definition ptr_minus (Γ : env Ti) (p1 p2 : ptr Ti) : Z :=
-    match p1, p2 with
-    | NULL _, NULL _ => 0
-    | Ptr a1, Ptr a2 => addr_minus Γ a1 a2
-    | _, _ => 0
-    end.
-  Global Arguments ptr_minus _ !_ !_ /.
-  Definition ptr_cast_ok (Γ : env Ti) (Γm : memenv Ti)
-      (σc : type Ti) (p : ptr Ti) : Prop :=
-    match p with NULL _ => True | Ptr a => addr_cast_ok Γ Γm σc a end.
-  Global Arguments ptr_cast_ok _ _ _ !_ /.
-  Definition ptr_cast (σc : type Ti) (p : ptr Ti) : ptr Ti :=
-    match p with NULL _ => NULL σc | Ptr a => Ptr (addr_cast σc a) end.
-  Global Arguments ptr_cast _ !_ /.
 
   Inductive ptr_refine' (Γ : env Ti) (f : meminj Ti) (Γm1 Γm2 : memenv Ti) :
        ptr Ti → ptr Ti → type Ti → Prop :=
@@ -158,74 +114,6 @@ Lemma ptr_dead_weaken Γ Γm1 Γm2 p σ :
 Proof. destruct 1; simpl; eauto using addr_dead_weaken. Qed.
 Global Instance ptr_alive_dec Γm p : Decision (ptr_alive Γm p).
 Proof. destruct p; apply _. Defined.
-Global Instance ptr_compare_ok_dec Γm c p1 p2 :
-  Decision (ptr_compare_ok Γm c p1 p2).
-Proof. destruct p1, p2, c; apply _. Defined.
-Global Instance ptr_plus_ok_dec Γ Γm j p : Decision (ptr_plus_ok Γ Γm j p).
-Proof. destruct p; apply _. Defined.
-Global Instance ptr_minus_ok_dec Γm p1 p2 : Decision (ptr_minus_ok Γm p1 p2).
-Proof. destruct p1, p2; apply _. Defined.
-Global Instance ptr_cast_ok_dec Γ Γm σc p : Decision (ptr_cast_ok Γ Γm σc p).
-Proof. destruct p; apply _. Defined.
-Lemma ptr_plus_typed Γ Γm p σ j :
-  ✓ Γ → (Γ,Γm) ⊢ p : σ → ptr_plus_ok Γ Γm j p → (Γ,Γm) ⊢ ptr_plus Γ j p : σ.
-Proof. destruct 2; simpl; constructor; eauto using addr_plus_typed. Qed.
-Lemma ptr_minus_typed Γ Γm p1 p2 σ :
-  ✓ Γ → (Γ,Γm) ⊢ p1 : σ → (Γ,Γm) ⊢ p2 : σ →
-  int_typed (ptr_minus Γ p1 p2) sptrT.
-Proof.
-  destruct 2, 1; simpl;
-    eauto using addr_minus_typed, int_typed_small with lia.
-Qed.
-Lemma ptr_cast_typed Γ Γm p σ σc :
-  (Γ,Γm) ⊢ p : σ → ptr_cast_ok Γ Γm σc p →
-  ptr_type_valid Γ σc → (Γ,Γm) ⊢ ptr_cast σc p : σc.
-Proof. destruct 1; simpl; constructor; eauto using addr_cast_typed. Qed.
-
-Lemma ptr_compare_ok_weaken Γm1 Γm2 c p1 p2 :
-  ptr_compare_ok Γm1 c p1 p2 → (∀ o, index_alive Γm1 o → index_alive Γm2 o) →
-  ptr_compare_ok Γm2 c p1 p2.
-Proof. destruct p1, p2, c; simpl; eauto using addr_minus_ok_weaken. Qed.
-Lemma ptr_compare_weaken Γ1 Γ2 Γm1 c p1 p2 τ1 τ2 :
-  ✓ Γ1 → (Γ1,Γm1) ⊢ p1 : τ1 → (Γ1,Γm1) ⊢ p2 : τ2 →
-  Γ1 ⊆ Γ2 → ptr_compare Γ1 c p1 p2 = ptr_compare Γ2 c p1 p2.
-Proof.
-  destruct 2,1,c; simpl; intros; done || by erewrite addr_minus_weaken by eauto.
-Qed.
-Lemma ptr_plus_ok_weaken Γ1 Γ2 Γm1 Γm2 p τ j :
-  ✓ Γ1 → (Γ1,Γm1) ⊢ p : τ → ptr_plus_ok Γ1 Γm1 j p →
-  Γ1 ⊆ Γ2 → (∀ o, index_alive Γm1 o → index_alive Γm2 o) →
-  ptr_plus_ok Γ2 Γm2 j p.
-Proof. destruct 2; simpl; eauto using addr_plus_ok_weaken. Qed.
-Lemma ptr_plus_weaken Γ1 Γ2 Γm1 p τ j :
-  ✓ Γ1 → (Γ1,Γm1) ⊢ p : τ → Γ1 ⊆ Γ2 → ptr_plus Γ1 j p = ptr_plus Γ2 j p.
-Proof. destruct 2; simpl; eauto using addr_plus_weaken, f_equal. Qed.
-Lemma ptr_minus_ok_weaken Γm1 Γm2 p1 p2:
-  ptr_minus_ok Γm1 p1 p2 → (∀ o, index_alive Γm1 o → index_alive Γm2 o) →
-  ptr_minus_ok Γm2 p1 p2.
-Proof. destruct p1, p2; simpl; eauto using addr_minus_ok_weaken. Qed.
-Lemma ptr_minus_weaken Γ1 Γ2 Γm1 p1 p2 τ1 τ2 :
-  ✓ Γ1 → (Γ1,Γm1) ⊢ p1 : τ1 → (Γ1,Γm1) ⊢ p2 : τ2 →
-  Γ1 ⊆ Γ2 → ptr_minus Γ1 p1 p2 = ptr_minus Γ2 p1 p2.
-Proof. destruct 2, 1; simpl; eauto using addr_minus_weaken. Qed.
-Lemma ptr_cast_ok_weaken Γ1 Γ2 Γm1 Γm2 p τ σc :
-  ✓ Γ1 → (Γ1,Γm1) ⊢ p : τ → ptr_cast_ok Γ1 Γm1 σc p → Γ1 ⊆ Γ2 →
-  (∀ o, index_alive Γm1 o → index_alive Γm2 o) → ptr_cast_ok Γ2 Γm2 σc p.
-Proof. destruct 2; simpl; eauto using addr_cast_ok_weaken. Qed.
-Lemma ptr_compare_ok_alive_l Γm c p1 p2 :
-  ptr_compare_ok Γm c p1 p2 → ptr_alive Γm p1.
-Proof. destruct p1, p2, c; try done; by intros [??]. Qed.
-Lemma ptr_compare_ok_alive_r Γm c p1 p2 :
-  ptr_compare_ok Γm c p1 p2 → ptr_alive Γm p2.
-Proof. destruct p1, p2, c; done || intros (?&?&?); simpl in *; congruence. Qed.
-Lemma ptr_plus_ok_alive Γ Γm p j : ptr_plus_ok Γ Γm j p → ptr_alive Γm p.
-Proof. destruct p. done. by intros [??]. Qed.
-Lemma ptr_minus_ok_alive_l Γm p1 p2 : ptr_minus_ok Γm p1 p2 → ptr_alive Γm p1.
-Proof. destruct p1, p2; try done. by intros [??]. Qed.
-Lemma ptr_minus_ok_alive_r Γm p1 p2 : ptr_minus_ok Γm p1 p2 → ptr_alive Γm p2.
-Proof. destruct p1, p2; try done. intros (?&?&?); simpl in *; congruence. Qed.
-Lemma ptr_cast_ok_alive Γ Γm p σ : ptr_cast_ok Γ Γm σ p → ptr_alive Γm p.
-Proof. destruct p. done. by intros [??]. Qed.
 
 (** ** Refinements *)
 Lemma ptr_refine_typed_l Γ f Γm1 Γm2 p1 p2 σ :
@@ -274,41 +162,4 @@ Proof. destruct 1; simpl; constructor; eauto using addr_freeze_refine. Qed.
 Lemma ptr_alive_refine Γ f Γm1 Γm2 p1 p2 σ :
   ptr_alive Γm1 p1 → p1 ⊑{Γ,f@Γm1↦Γm2} p2 : σ → ptr_alive Γm2 p2.
 Proof. destruct 2; simpl in *; eauto using addr_alive_refine. Qed.
-Lemma ptr_compare_ok_refine Γ Γm1 Γm2 f c p1 p2 p3 p4 σ :
-  p1 ⊑{Γ,f@Γm1↦Γm2} p2 : σ → p3 ⊑{Γ,f@Γm1↦Γm2} p4 : σ →
-  ptr_compare_ok Γm1 c p1 p3 → ptr_compare_ok Γm2 c p2 p4.
-Proof.
-  destruct 1, 1, c; simpl; eauto using addr_minus_ok_refine, addr_alive_refine.
-Qed.
-Lemma ptr_compare_refine Γ f Γm1 Γm2 c p1 p2 p3 p4 σ :
-  ✓ Γ → ptr_compare_ok Γm1 c p1 p3 →
-  p1 ⊑{Γ,f@Γm1↦Γm2} p2 : σ → p3 ⊑{Γ,f@Γm1↦Γm2} p4 : σ →
-  ptr_compare Γ c p1 p3 = ptr_compare Γ c p2 p4.
-Proof.
-  destruct 3, 1, c; simpl; done || by erewrite addr_minus_refine by eauto.
-Qed.
-Lemma ptr_plus_ok_refine Γ Γm1 Γm2 f p1 p2 σ j :
-  p1 ⊑{Γ,f@Γm1↦Γm2} p2 : σ → ptr_plus_ok Γ Γm1 j p1 → ptr_plus_ok Γ Γm2 j p2.
-Proof. destruct 1; simpl; eauto using addr_plus_ok_refine. Qed.
-Lemma ptr_plus_refine Γ f Γm1 Γm2 p1 p2 σ j :
-  ✓ Γ → ptr_plus_ok Γ Γm1 j p1 →
-  p1 ⊑{Γ,f@Γm1↦Γm2} p2 : σ → ptr_plus Γ j p1 ⊑{Γ,f@Γm1↦Γm2} ptr_plus Γ j p2 : σ.
-Proof. destruct 3; simpl; constructor; eauto using addr_plus_refine. Qed.
-Lemma ptr_minus_ok_refine Γ Γm1 Γm2 f p1 p2 p3 p4 σ :
-  p1 ⊑{Γ,f@Γm1↦Γm2} p2 : σ → p3 ⊑{Γ,f@Γm1↦Γm2} p4 : σ →
-  ptr_minus_ok Γm1 p1 p3 → ptr_minus_ok Γm2 p2 p4.
-Proof. destruct 1, 1; simpl; eauto using addr_minus_ok_refine. Qed.
-Lemma ptr_minus_refine Γ f Γm1 Γm2 p1 p2 p3 p4 σ :
-  ✓ Γ → ptr_minus_ok Γm1 p1 p3 →
-  p1 ⊑{Γ,f@Γm1↦Γm2} p2 : σ → p3 ⊑{Γ,f@Γm1↦Γm2} p4 : σ →
-  ptr_minus Γ p1 p3 = ptr_minus Γ p2 p4.
-Proof. destruct 3, 1; simpl; eauto using addr_minus_refine. Qed.
-Lemma ptr_cast_ok_refine Γ f Γm1 Γm2 p1 p2 σ σc :
-  ✓ Γ → p1 ⊑{Γ,f@Γm1↦Γm2} p2 : σ →
-  ptr_cast_ok Γ Γm1 σc p1 → ptr_cast_ok Γ Γm2 σc p2.
-Proof. destruct 2; simpl; eauto using addr_cast_ok_refine. Qed.
-Lemma ptr_cast_refine Γ f Γm1 Γm2 p1 p2 σ σc :
-  ptr_cast_ok Γ Γm1 σc p1 → ptr_type_valid Γ σc → p1 ⊑{Γ,f@Γm1↦Γm2} p2 : σ →
-  ptr_cast σc p1 ⊑{Γ,f@Γm1↦Γm2} ptr_cast σc p2 : σc.
-Proof. destruct 3; constructor; eauto using addr_cast_refine. Qed.
 End pointers.
