aliasing.v
@@ -1,0 +1,182 @@
+(* Copyright (c) 2012-2014, Robbert Krebbers. *)
+(* This file is distributed under the terms of the BSD license. *)
+Require Export operations memory.
+
+Section aliasing.
+Context `{EnvSpec Ti}.
+Implicit Types Γ : env Ti.
+Implicit Types Γm : memenv Ti.
+Implicit Types τ σ : type Ti.
+Implicit Types r : ref Ti.
+Implicit Types a : addr Ti.
+Implicit Types w : mtree Ti.
+Implicit Types v : val Ti.
+Implicit Types m : mem Ti.
+Arguments lookupE _ _ _ _ _ _ _ !_ /.
+Arguments cmap_lookup _ _ _ _ !_ /.
+
+Lemma ref_disjoint_cases Γ τ r1 r2 σ1 σ2 :
+  ✓ Γ → Γ ⊢ r1 : τ ↣ σ1 → freeze true <$> r1 = r1 →
+  Γ ⊢ r2 : τ ↣ σ2 → freeze true <$> r2 = r2 →
+  (**i 1.) *) (∀ j1 j2, ref_set_offset j1 r1 ⊥ ref_set_offset j2 r2) ∨
+  (**i 2.) *) σ1 ⊆{Γ} σ2 ∨
+  (**i 3.) *) σ2 ⊆{Γ} σ1 ∨
+  (**i 4.) *) ∃ s r1' i1 r2' i2 r', r1 = r1' ++ RUnion i1 s true :: r' ∧
+    r2 = r2' ++ RUnion i2 s true :: r' ∧ i1 ≠ i2.
+Proof.
+  intros HΓ Hr1 Hr1F Hr2 Hr2F. cut (
+    (**i 1.) *) (∀ j1 j2, ref_set_offset j1 r1 ⊥ ref_set_offset j2 r2) ∨
+    (**i 2.) *) (∃ j r', r1 = r' ++ ref_set_offset j r2) ∨
+    (**i 3.) *) (∃ j r', r2 = r' ++ ref_set_offset j r1) ∨
+    (**i 4.) *) ∃ s r1' i1 r2' i2 r', r1 = r1' ++ [RUnion i1 s true] ++ r' ∧
+      r2 = r2' ++ [RUnion i2 s true] ++ r' ∧ i1 ≠ i2).
+  { intros [?|[(j&r'&->)|[(j&r'&->)|(s&r1'&i1&r2'&i2&r'&Hr1'&Hr2'&?)]]].
+    * by left.
+    * rewrite ref_typed_app in Hr1; destruct Hr1 as (σ2'&?&?).
+      assert (σ2'=σ2) as -> by eauto using ref_set_offset_typed_unique, eq_sym.
+      by right; left; exists r'.
+    * rewrite ref_typed_app in Hr2; destruct Hr2 as (σ1'&?&?).
+      assert (σ1'=σ1) as -> by eauto using ref_set_offset_typed_unique, eq_sym.
+      by do 2 right; left; exists r'.
+    * do 3 right; naive_solver. }
+  revert r1 τ σ1 Hr1 r2 σ2 Hr1F Hr2 Hr2F. assert (∀ τ rs1 r2 σ1 σ2,
+    Γ ⊢ rs1 : τ ↣ σ1 → freeze true rs1 = rs1 →
+    Γ ⊢ r2 : τ ↣ σ2 → freeze true <$> r2 = r2 →
+    (* 1.) *) (∀ j1 j2, ref_set_offset j1 [rs1] ⊥ ref_set_offset j2 r2) ∨
+    (* 2.) *) (∃ j r', r2 = r' ++ ref_set_offset j [rs1]) ∨
+    (* 3.) *) r2 = [] ∨
+    (* 4.) *) ∃ s i1 r2' i2, rs1 = RUnion i1 s true ∧
+      r2 = r2' ++ [RUnion i2 s true] ∧ i1 ≠ i2) as aux.
+  { intros τ rs1 r2 σ1 σ2 Hrs1 Hrs1F Hr2 Hr2F.
+    destruct r2 as [|rs2 r2 _] using rev_ind; [by do 2 right; left|].
+    rewrite ref_typed_snoc in Hr2; destruct Hr2 as (σ2'&Hrs2&Hr2).
+    rewrite fmap_app in Hr2F. destruct Hrs1 as [? i1 n|s i1|s i1 ?];
+      inversion Hrs2 as [? i2|? i2|? i2 []]; simplify_list_equality.
+    * by right; left; exists i2 r2.
+    * destruct (decide (i1 = i2)) as [->|]; [by right; left; exists 0 r2|].
+      left. intros _ ?. destruct r2; simpl; [by repeat constructor|].
+      rewrite app_comm_cons. apply ref_disjoint_app_r. by repeat constructor.
+    * destruct (decide (i1 = i2)) as [->|]; [by right; left; exists 0 r2|].
+      do 3 right. by exists s i1 r2 i2. }
+  induction 1 as [τ|r1 rs1 τ τ1 σ1 Hrs1 Hr1 IH]
+    using @ref_typed_ind; intros r2 σ2 Hr1F Hr2 Hr2F; simplify_equality'.
+  { do 2 right; left; exists 0 r2. by rewrite (right_id_L [] (++)). }
+  destruct Hr2 as [τ|r2 rs2 τ τ2 σ2 Hrs2 Hr2 _]
+    using @ref_typed_ind; simplify_equality'.
+  { right; left; exists 0 (rs1 :: r1). by rewrite (right_id_L [] (++)). }
+  destruct (IH r2 τ2) as
+    [Hr|[(j&r'&->)|[(j&r'&->)|(s&r1'&i1&r2'&i2&r'&->&->&?)]]];
+    auto; clear IH; simplify_equality'.
+  * left; intros j1 j2. apply ref_disjoint_cons_l, ref_disjoint_cons_r.
+    by rewrite <-(ref_set_offset_offset r1), <-(ref_set_offset_offset r2).
+  * rewrite ref_typed_app in Hr1; destruct Hr1 as (τ2'&Hr2'&Hr').
+    assert (τ2' = τ2) as -> by eauto using ref_set_offset_typed_unique, eq_sym.
+    destruct (ref_set_offset_disjoint r2 j) as [?| ->].
+    { left; intros j1 j2. rewrite app_comm_cons.
+      by apply ref_disjoint_app_l, ref_disjoint_cons_r. }
+    destruct (aux τ2 rs2 (rs1 :: r') σ2 σ1)
+      as [Hr|[(j'&r''&Hr'')|[?|(s&i1&r2'&i2&?&Hr2''&?)]]];
+      simplify_equality'; auto.
+    { econstructor; eauto. }
+    { destruct (app_injective_1 (freeze true <$> r') r'
+        (freeze true <$> ref_set_offset j r2) (ref_set_offset j r2));
+        rewrite ?fmap_length, <-?fmap_app; congruence. }
+    + left; intros j1 j2. rewrite app_comm_cons.
+      apply (ref_disjoint_here_app _ [_]), symmetry, Hr.
+    + right; left; exists j' r''.
+      by rewrite app_comm_cons, Hr'', <-(associative_L (++)).
+    + do 3 right. eexists s, r2', i2, [], i1, r2.
+      by rewrite app_comm_cons, Hr2'', <-(associative_L (++)).
+  * rewrite ref_typed_app in Hr2; destruct Hr2 as (τ1'&Hr1'&Hr').
+    assert (τ1' = τ1) as -> by eauto using ref_set_offset_typed_unique, eq_sym.
+    destruct (ref_set_offset_disjoint r1 j) as [?| ->]; simpl.
+    { left; intros. rewrite app_comm_cons. by apply (ref_disjoint_app [_]). }
+    destruct (aux τ1 rs1 (rs2 :: r') σ1 σ2)
+      as [Hr|[(j'&r''&Hr'')|[?|(s&i1&r2'&i2&?&Hr1''&?)]]];
+      simplify_equality'; auto.
+    { econstructor; eauto. }
+    { destruct (app_injective_1 (freeze true <$> r') r'
+        (freeze true <$> ref_set_offset j r1) (ref_set_offset j r1));
+        rewrite ?fmap_length, <-?fmap_app; congruence. }
+    + left; intros j1 j2. rewrite app_comm_cons.
+      apply (ref_disjoint_here_app [_]), Hr.
+    + do 2 right; left; exists j' r''.
+      by rewrite app_comm_cons, Hr'', <-(associative_L (++)).
+    + do 3 right; eexists s, [], i1, r2', i2, r1.
+      by rewrite app_comm_cons, Hr1'', <-(associative_L (++)).
+  * by do 3 right; eexists s, (rs1 :: r1'), i1, (rs2 :: r2'), i2, r'.
+Qed.
+Lemma addr_disjoint_cases Γ Γm a1 a2 σ1 σ2 :
+  ✓ Γ → (Γ,Γm) ⊢ a1 : σ1 → frozen a1 → addr_is_obj a1 →
+  (Γ,Γm) ⊢ a2 : σ2 → frozen a2 → addr_is_obj a2 →
+  (**i 1.) *) (∀ j1 j2, addr_plus Γ j1 a1 ⊥{Γ} addr_plus Γ j2 a2) ∨
+  (**i 2.) *) σ1 ⊆{Γ} σ2 ∨
+  (**i 3.) *) σ2 ⊆{Γ} σ1 ∨
+  (**i 4.) *) addr_index a1 = addr_index a2 ∧ (∃ s r1' i1 r2' i2 r',
+    addr_ref_base a1 = r1' ++ RUnion i1 s true :: r' ∧
+    addr_ref_base a2 = r2' ++ RUnion i2 s true :: r' ∧ i1 ≠ i2).
+Proof.
+  unfold frozen. intros ? [o1 r1 i1 τ1 σ1' σc1] ??
+    [o2 r2 i2 τ2 σ2' σc2] ??; simplify_equality'.
+  destruct (decide (o1 = o2)); [simplify_type_equality|by do 2 left].
+  destruct (ref_disjoint_cases Γ τ2 r1 r2 σ1' σ2')
+    as [?|[?|[?|(s&r1'&i1'&r2'&i2'&r'&->&->&?)]]]; auto.
+  * left; intros j1 j2; right; left; split; simpl; auto.
+  * do 3 right; split; [done|]. by eexists s, r1', i1', r2', i2', r'.
+Qed.
+Lemma cmap_non_aliasing Γ Γm m a1 a2 σ1 σ2 :
+  ✓ Γ → ✓{Γ,Γm} m → (Γ,Γm) ⊢ a1 : σ1 → frozen a1 → addr_is_obj a1 →
+  (Γ,Γm) ⊢ a2 : σ2 → frozen a2 → addr_is_obj a2 →
+  (**i 1.) *) (∀ j1 j2, addr_plus Γ j1 a1 ⊥{Γ} addr_plus Γ j2 a2) ∨
+  (**i 2.) *) σ1 ⊆{Γ} σ2 ∨
+  (**i 3.) *) σ2 ⊆{Γ} σ1 ∨
+  (**i 4.) *) ∀ g j1 j2,
+    cmap_alter Γ g (addr_plus Γ j1 a1) m !!{Γ} addr_plus Γ j2 a2 
+    = @None (mtree _) ∧
+    cmap_alter Γ g (addr_plus Γ j2 a2) m !!{Γ} addr_plus Γ j1 a1
+    = @None (mtree _).
+Proof.
+  intros ? Hm ??????. destruct (addr_disjoint_cases Γ Γm a1 a2 σ1 σ2)
+    as [Ha12|[?|[?|(Hidx&s&r1'&i1&r2'&i2&r'&Ha1&Ha2&?)]]]; auto.
+  do 3 right. intros g j1 j2.
+  assert (Γm ⊢ addr_index a1 : addr_type_object a1)
+    by eauto using addr_typed_index.
+  assert (Γm ⊢ addr_index a1 : addr_type_object a2)
+    by (rewrite Hidx; eauto using addr_typed_index).
+  destruct m as [m]; unfold insertE, cmap_alter, lookupE, cmap_lookup;
+    simpl in *; rewrite !addr_index_plus, <-!Hidx; simplify_map_equality'.
+  destruct (m !! addr_index a1) as [[|w malloc]|] eqn:?;
+    [by simplify_option_equality| |by simplify_option_equality].
+  destruct (proj2 Hm (addr_index a1) w malloc)
+    as (τ&?&_&?&_); auto; simplify_type_equality'.
+  assert (Γ ⊢ r1' ++ RUnion i1 s true :: r' :
+    addr_type_object a2 ↣ addr_type_base a1).
+  { erewrite <-Ha1, <-(typed_unique _ (addr_index a1)
+      (addr_type_object a1) (addr_type_object a2)) by eauto.
+    eauto using addr_typed_ref_base_typed. }
+  assert (Γ ⊢ r2' ++ RUnion i2 s true :: r' :
+    addr_type_object a2 ↣ addr_type_base a2).
+  { rewrite <-Ha2. eauto using addr_typed_ref_base_typed. }
+  unfold addr_ref; rewrite !addr_ref_base_plus, Ha1, Ha2.
+  by split; case_option_guard; simplify_equality;
+    erewrite ?ctree_lookup_non_aliasing by eauto.
+Qed.
+Lemma mem_non_aliasing Γ Γm m a1 a2 τ1 τ2 :
+  ✓ Γ → ✓{Γ,Γm} m → (Γ,Γm) ⊢ a1 : τ1 → frozen a1 → addr_is_obj a1 →
+  (Γ,Γm) ⊢ a2 : τ2 → frozen a2 → addr_is_obj a2 →
+  (**i 1.) *) (∀ j1 j2, addr_plus Γ j1 a1 ⊥{Γ} addr_plus Γ j2 a2) ∨
+  (**i 2.) *) τ1 ⊆{Γ} τ2 ∨
+  (**i 3.) *) τ2 ⊆{Γ} τ1 ∨
+  (**i 4.) *) ∀ j1 j2,
+    (∀ v1, <[addr_plus Γ j1 a1:=v1]{Γ}>m !!{Γ} addr_plus Γ j2 a2 = None) ∧
+    mem_force Γ (addr_plus Γ j1 a1) m !!{Γ} addr_plus Γ j2 a2 = None ∧
+    (∀ v2, <[addr_plus Γ j2 a2:=v2]{Γ}>m !!{Γ} addr_plus Γ j1 a1 = None) ∧
+    mem_force Γ (addr_plus Γ j2 a2) m !!{Γ} addr_plus Γ j1 a1 = None.
+Proof.
+  intros.
+  destruct (cmap_non_aliasing Γ Γm m a1 a2 τ1 τ2) as [?|[?|[?|Ha]]]; auto.
+  unfold lookupE, mem_lookup, insertE, mem_insert, mem_force.
+  by do 3 right; repeat split; intros;
+    rewrite ?(proj1 (Ha _ _ _)), ?(proj2 (Ha _ _ _)).
+Qed.
+End aliasing.
