operations.v
@@ -1,0 +1,1193 @@
+(* Copyright (c) 2012-2014, Robbert Krebbers. *)
+(* This file is distributed under the terms of the BSD license. *)
+Require Export memory_map values.
+Require Import pointer_casts.
+Local Open Scope ctype_scope.
+
+Section operations.
+  Context `{Env Ti}.
+
+  (** ** Operations on addresses *)
+  Definition addr_plus_ok (Γ : env Ti) (Γm : memenv Ti)
+      (j : Z) (a : addr Ti) : Prop :=
+    index_alive Γm (addr_index a) ∧
+    (0 ≤ addr_byte a + j * size_of' Γ a
+       ≤ size_of Γ (addr_type_base a) * ref_size (addr_ref_base a))%Z.
+  Global Arguments addr_plus_ok _ _ _ !_ /.
+  Definition addr_plus (Γ : env Ti) (j : Z) (a : addr Ti): addr Ti :=
+    let 'Addr x r i τ σ σc := a
+    in Addr x r (Z.to_nat (i + j * size_of Γ σc)) τ σ σc.
+  Global Arguments addr_plus _ _ !_ /.
+
+  Definition addr_minus_ok (Γm : memenv Ti) (a1 a2 : addr Ti) : Prop :=
+    index_alive Γm (addr_index a1) ∧
+    addr_index a1 = addr_index a2 ∧
+    freeze true <$> addr_ref_base a1 = freeze true <$> addr_ref_base a2.
+  Global Arguments addr_minus_ok _ !_ !_ /.
+  Definition addr_minus (Γ : env Ti) (a1 a2 : addr Ti) : Z :=
+    ((addr_byte a1 - addr_byte a2) `div` size_of' Γ a1)%Z.
+  Global Arguments addr_minus _ !_ !_ /.
+
+  Definition addr_cast_ok (Γ : env Ti) (Γm : memenv Ti)
+      (σc : type Ti) (a : addr Ti) : Prop :=
+    index_alive Γm (addr_index a) ∧
+    addr_type_base a >*> σc ∧
+    addr_byte a `mod` size_of Γ σc = 0.
+  Global Arguments addr_cast_ok _ _ _ !_ /.
+  Definition addr_cast (σc : type Ti) (a : addr Ti) : addr Ti :=
+    let 'Addr o r i τ σ _ := a in Addr o r i τ σ σc.
+  Global Arguments addr_cast _ !_ /.
+
+  Definition addr_elt (Γ : env Ti) (rs : ref_seg Ti) (a : addr Ti) : addr Ti :=
+    from_option a $
+     σ ← type_of a !!{Γ} rs;
+     Some (Addr (addr_index a) (rs :: addr_ref Γ a) 0 (addr_type_object a) σ σ).
+  Global Arguments addr_elt _ _ !_ /.
+
+  (** ** Operations on pointers *)
+  Definition ptr_compare_ok (Γm : memenv Ti) (c : compop) (p1 p2 : ptr Ti) : Prop :=
+    match p1, p2 with
+    | Ptr a1, Ptr a2 => addr_minus_ok Γm a1 a2
+    | NULL _, Ptr a2 =>
+       match c with EqOp => index_alive Γm (addr_index a2) | _ => False end
+    | Ptr a1, NULL _ =>
+       match c with EqOp => index_alive Γm (addr_index a1) | _ => False end
+    | NULL _, NULL _ => True
+    end.
+  Definition ptr_compare (Γ : env Ti) (c : compop) (p1 p2 : ptr Ti) : bool :=
+    match p1, p2 with
+    | Ptr a1, Ptr a2 => Z_comp c (addr_minus Γ a1 a2) 0
+    | NULL _, Ptr a2 => false (* only allowed for EqOp *)
+    | Ptr a1, NULL _ => false (* only allowed for EqOp *)
+    | NULL _, NULL _ => match c with EqOp | LeOp => true | LtOp => false end
+    end.
+  Definition ptr_plus_ok (Γ : env Ti) (Γm : memenv Ti) (j : Z) (p : ptr Ti) :=
+    match p with NULL _ => j = 0 | Ptr a => addr_plus_ok Γ Γm j a end.
+  Global Arguments ptr_plus_ok _ _ _ !_ /.
+  Definition ptr_plus (Γ : env Ti) (j : Z) (p : ptr Ti) : ptr Ti :=
+    match p with NULL τ => NULL τ | Ptr a => Ptr (addr_plus Γ j a) end.
+  Global Arguments ptr_plus _ _ !_ /.
+  Definition ptr_minus_ok (Γm : memenv Ti) (p1 p2 : ptr Ti) : Prop :=
+    match p1, p2 with
+    | NULL _, NULL _ => True
+    | Ptr a1, Ptr a2 => addr_minus_ok Γm a1 a2
+    | _, _ => False
+    end.
+  Global Arguments ptr_minus_ok _ !_ !_ /.
+  Definition ptr_minus (Γ : env Ti) (p1 p2 : ptr Ti) : Z :=
+    match p1, p2 with
+    | NULL _, NULL _ => 0
+    | Ptr a1, Ptr a2 => addr_minus Γ a1 a2
+    | _, _ => 0
+    end.
+  Global Arguments ptr_minus _ !_ !_ /.
+  Definition ptr_cast_ok (Γ : env Ti) (Γm : memenv Ti)
+      (σc : type Ti) (p : ptr Ti) : Prop :=
+    match p with NULL _ => True | Ptr a => addr_cast_ok Γ Γm σc a end.
+  Global Arguments ptr_cast_ok _ _ _ !_ /.
+  Definition ptr_cast (σc : type Ti) (p : ptr Ti) : ptr Ti :=
+    match p with NULL _ => NULL σc | Ptr a => Ptr (addr_cast σc a) end.
+  Global Arguments ptr_cast _ !_ /.  
+
+  (** ** Operations on base values *)
+  Definition base_val_true (Γm : memenv Ti) (vb : base_val Ti) : Prop :=
+    match vb with
+    | VInt _ x => x ≠ 0
+    | VPtr (Ptr a) => index_alive Γm (addr_index a)
+    | _ => False
+    end.
+  Definition base_val_false (vb : base_val Ti) : Prop :=
+    match vb with VInt _ x => x = 0 | VPtr (NULL _) => True | _ => False end.
+  Definition base_val_0 (τb : base_type Ti) : base_val Ti :=
+    match τb with
+    | voidT => VVoid | intT τi => VInt τi 0 | τ.* => VPtr (NULL τ)
+    end%BT.
+
+  Inductive base_unop_typed : unop → base_type Ti → base_type Ti → Prop :=
+    | TInt_NegOp_typed τi :
+       base_unop_typed NegOp (intT τi) (intT (int_promote τi))
+    | TInt_ComplOp_typed τi :
+       base_unop_typed ComplOp (intT τi) (intT (int_promote τi))
+    | TInt_NotOp_typed τi :
+       base_unop_typed NotOp (intT τi) sintT
+    | TPtr_NotOp_typed τ : base_unop_typed NotOp (τ.*) sintT.
+  Definition base_unop_type_of (op : unop)
+      (τb : base_type Ti) : option (base_type Ti) :=
+    match τb, op with
+    | intT τi, NotOp => Some sintT
+    | intT τi, _ => Some (intT (int_promote τi))
+    | τ.*, NotOp => Some sintT
+    | _, _ => None
+    end%BT.
+  Definition base_val_unop_ok (Γm : memenv Ti)
+      (op : unop) (vb : base_val Ti) : Prop :=
+    match vb, op with
+    | VInt τi x, NegOp => int_arithop_ok MinusOp 0 τi x τi
+    | VInt τi x, _ => True
+    | VPtr p, NotOp => ptr_alive Γm p
+    | _, _ => False
+    end.
+  Global Arguments base_val_unop_ok _ !_ !_ /.
+  Definition base_val_unop (op : unop) (vb : base_val Ti) : base_val Ti :=
+    match vb, op with
+    | VInt τi x, NegOp => VInt (int_promote τi) (int_arithop MinusOp 0 τi x τi)
+    | VInt τi x, ComplOp =>
+       let τi' := int_promote τi in
+       VInt τi' (int_of_bits τi' (negb <$> int_to_bits τi' x))
+    | VInt τi x, NotOp => VInt sintT (if decide (x = 0) then 1 else 0)
+    | VPtr p, _ => VInt sintT (match p with NULL _ => 1 | Ptr _ => 0 end)
+    | _, _ => vb
+    end.
+  Global Arguments base_val_unop !_ !_ /.
+
+  Inductive base_binop_typed :
+        binop → base_type Ti → base_type Ti → base_type Ti → Prop :=
+    | CompOp_TInt_TInt_typed op τi1 τi2 :
+       base_binop_typed (CompOp op) (intT τi1) (intT τi2) sintT
+    | ArithOp_TInt_TInt_typed op τi1 τi2 :
+       base_binop_typed (ArithOp op) (intT τi1) (intT τi2)
+         (intT (int_promote τi1 ∪ int_promote τi2))
+    | ShiftOp_TInt_TInt_typed op τi1 τi2 :
+       base_binop_typed (ShiftOp op) (intT τi1) (intT τi2)
+         (intT (int_promote τi1))
+    | BitOp_TInt_TInt_typed op τi1 τi2 :
+       base_binop_typed (BitOp op) (intT τi1) (intT τi2)
+         (intT (int_promote τi1 ∪ int_promote τi2))
+    | CompOp_TPtr_TPtr_typed c τ :
+       base_binop_typed (CompOp c) (τ.*) (τ.*) sintT
+    | PlusOp_TPtr_TInt_typed τ σ :
+       base_binop_typed (ArithOp PlusOp) (τ.*) (intT σ) (τ.*)
+    | PlusOp_VInt_TPtr_typed τ σ :
+       base_binop_typed (ArithOp PlusOp) (intT σ) (τ.*) (τ.*)
+    | MinusOp_TPtr_TInt_typed τ σi :
+       base_binop_typed (ArithOp MinusOp) (τ.*) (intT σi) (τ.*)
+    | MinusOp_TInt_TPtr_typed τ σi :
+       base_binop_typed (ArithOp MinusOp) (intT σi) (τ.*) (τ.*)
+    | MinusOp_TPtr_TPtr_typed τ  :
+       base_binop_typed (ArithOp MinusOp) (τ.*) (τ.*) sptrT.
+  Definition base_binop_type_of
+      (op : binop) (τb1 τb2 : base_type Ti) : option (base_type Ti) :=
+    match τb1, τb2, op with
+    | intT τi1, intT τi2, CompOp _ => Some sintT
+    | intT τi1, intT τi2, (ArithOp _ | BitOp _) =>
+       Some (intT (int_promote τi1 ∪ int_promote τi2))
+    | intT τi1, intT τi2, ShiftOp _ => Some (intT (int_promote τi1))
+    | τ1.*, τ2.*, CompOp _ => guard (τ1 = τ2); Some sintT
+    | τ.*, intT σ, (ArithOp PlusOp | ArithOp MinusOp) => Some (τ.*)
+    | intT σ, τ.*, (ArithOp PlusOp | ArithOp MinusOp) => Some (τ.*)
+    | τ1.*, τ2.*, ArithOp MinusOp => guard (τ1 = τ2); Some sptrT
+    | _, _, _ => None
+    end%BT.
+  Definition base_val_binop_ok (Γ : env Ti) (Γm : memenv Ti)
+      (op : binop) (vb1 vb2 : base_val Ti) : Prop :=
+    match vb1, vb2, op with
+    | VInt τi1 x1, VInt τi2 x2, (CompOp _ | BitOp _) => True
+    | VInt τi1 x1, VInt τi2 x2, ArithOp op => int_arithop_ok op x1 τi1 x2 τi2
+    | VInt τi1 x1, VInt τi2 x2, ShiftOp op => int_shiftop_ok op x1 τi1 x2 τi2
+    | VPtr p1, VPtr p2, CompOp c => ptr_compare_ok Γm c p1 p2
+    | VPtr p, VInt _ x, ArithOp PlusOp => ptr_plus_ok Γ Γm x p
+    | VInt _ x, VPtr p, ArithOp PlusOp => ptr_plus_ok Γ Γm x p
+    | VPtr p, VInt _ x, ArithOp MinusOp => ptr_plus_ok Γ Γm (-x) p
+    | VInt _ x, VPtr p, ArithOp MinusOp => ptr_plus_ok Γ Γm (-x) p
+    | VPtr p1, VPtr p2, ArithOp MinusOp => ptr_minus_ok Γm p1 p2
+    | _, _, _ => False
+    end.
+  Global Arguments base_val_binop_ok _ _ !_ !_ !_ /.
+  Definition base_val_binop (Γ : env Ti)
+      (op : binop) (v1 v2 : base_val Ti) : base_val Ti :=
+    match v1, v2, op with
+    | VInt τi1 x1, VInt τi2 x2, CompOp op =>
+       let τi' := int_promote τi1 ∪ int_promote τi2 in
+       let x1' := int_cast τi' x1 in let x2' := int_cast τi' x2 in
+       VInt sintT (if Z_comp op x1' x2' then 1 else 0)
+    | VInt τi1 x1, VInt τi2 x2, ArithOp op =>
+       VInt (int_promote τi1 ∪ int_promote τi2) (int_arithop op x1 τi1 x2 τi2)
+    | VInt τi1 x1, VInt τi2 x2, ShiftOp op =>
+       VInt (int_promote τi1) (int_shiftop op x1 τi1 x2 τi2)
+    | VInt τi1 x1, VInt τi2 x2, BitOp op =>
+       let τi' := int_promote τi1 ∪ int_promote τi2 in
+       VInt τi' (int_of_bits τi'
+         (zip_with (bool_bitop op) (int_to_bits τi' x1) (int_to_bits τi' x2)))
+    | VPtr p1, VPtr p2, CompOp c =>
+       VInt sintT (if ptr_compare Γ c p1 p2 then 1 else 0)
+    | VPtr p, VInt _ i, ArithOp PlusOp => VPtr (ptr_plus Γ i p)
+    | VInt _ i, VPtr p, ArithOp PlusOp => VPtr (ptr_plus Γ i p)
+    | VPtr p, VInt _ i, ArithOp MinusOp => VPtr (ptr_plus Γ (-i) p)
+    | VInt _ i, VPtr p, ArithOp MinusOp => VPtr (ptr_plus Γ (-i) p)
+    | VPtr p1, VPtr p2, ArithOp MinusOp => VInt sptrT (ptr_minus Γ p1 p2)
+    | _, _, _ => VIndet (type_of v1)
+    end.
+  Global Arguments base_val_binop _ !_ !_ !_ /.
+
+  Inductive base_cast_typed (Γ : env Ti) :
+       base_type Ti → base_type Ti → Prop :=
+    | TVoid_cast_typed τb : base_cast_typed Γ τb voidT
+    | TInt_cast_typed τi1 τi2 : base_cast_typed Γ (intT τi1) (intT τi2)
+    | TPtr_to_TPtr_cast_typed τ : base_cast_typed Γ (τ.*) (τ.*)
+    | TPtr_to_void_cast_typed τ : base_cast_typed Γ (τ.*) (voidT.*)
+    | TPtr_to_uchar_cast_typed τ : base_cast_typed Γ (τ.*) (ucharT.*)
+    | TPtr_of_void_cast_typed τ :
+       ptr_type_valid Γ τ → base_cast_typed Γ (voidT.*) (τ.*)
+    | TPtr_of_uchar_cast_typed τ :
+       ptr_type_valid Γ τ → base_cast_typed Γ (ucharT.*) (τ.*).
+  Definition base_val_cast_ok (Γ : env Ti) (Γm : memenv Ti)
+      (τb : base_type Ti) (vb : base_val Ti) : Prop :=
+    match vb, τb with
+    | (VVoid | VInt _ _ | VByte _), voidT => True
+    | VIndet τi, voidT => τi = ucharT
+    | VPtr p, voidT => ptr_alive Γm p
+    | VInt _ x, intT τi => int_cast_ok τi x
+    | VPtr p, τ.* => ptr_cast_ok Γ Γm τ p
+    | VByte _, intT τi => τi = ucharT%IT
+    | VIndet τi, intT τi' => τi = ucharT ∧ τi' = ucharT%IT
+    | _, _ => False
+    end%BT.
+  Global Arguments base_val_cast_ok _ _ !_ !_ /.
+  Definition base_val_cast (τb : base_type Ti)
+      (vb : base_val Ti) : base_val Ti :=
+    match vb, τb with
+    | _, voidT => VVoid
+    | VInt _ x, intT τi => VInt τi (int_cast τi x)
+    | VPtr p, τ.* => VPtr (ptr_cast τ p)
+    | _ , _ => vb
+    end%BT.
+  Global Arguments base_val_cast !_ !_ /.
+
+  (** ** Operations on values *)
+  Definition val_0 (Γ : env Ti) : type Ti → val Ti := type_iter
+    (**i TBase     *) (λ τb, VBase (base_val_0 τb))
+    (**i TArray    *) (λ τ n x, VArray τ (replicate n x))
+    (**i TCompound *) (λ c s τs rec,
+      match c with
+      | Struct_kind => VStruct s (rec <$> τs)
+      | Union_kind => VUnion s 0 (default (VUnionAll s []) (τs !! 0) rec)
+      end) Γ.
+
+  Definition val_true (Γm : memenv Ti) (v : val Ti) : Prop :=
+    match v with VBase vb => base_val_true Γm vb | _ => False end.
+  Definition val_false (v : val Ti) : Prop :=
+    match v with VBase vb => base_val_false vb | _ => False end.
+
+  Inductive unop_typed : unop → type Ti → type Ti → Prop :=
+    | TBase_unop_typed op τb σb :
+       base_unop_typed op τb σb → unop_typed op (baseT τb) (baseT σb).
+  Definition unop_type_of (op : unop) (τ : type Ti) : option (type Ti) :=
+    match τ with
+    | baseT τb => σb ← base_unop_type_of op τb; Some (baseT σb) | _ => None
+    end.
+  Definition val_unop_ok (Γm : memenv Ti) (op : unop) (v : val Ti) : Prop :=
+    match v with VBase vb => base_val_unop_ok Γm op vb | _ => False end.
+  Global Arguments val_unop_ok _ !_ !_ /.
+  Definition val_unop (op : unop) (v : val Ti) : val Ti :=
+    match v with VBase vb => VBase (base_val_unop op vb) | _ => v end.
+  Global Arguments val_unop !_ !_ /.
+
+  Inductive binop_typed : binop → type Ti → type Ti → type Ti → Prop :=
+    | TBase_binop_typed op τb1 τb2 σb :
+       base_binop_typed op τb1 τb2 σb →
+       binop_typed op (baseT τb1) (baseT τb2) (baseT σb).
+  Definition binop_type_of (op : binop) (τ1 τ2 : type Ti) : option (type Ti) :=
+    match τ1, τ2 with
+    | baseT τb1, baseT τb2 =>
+       σb ← base_binop_type_of op τb1 τb2; Some (baseT σb)
+    | _, _ => None
+    end.
+  Definition val_binop_ok (Γ : env Ti) (Γm : memenv Ti)
+      (op : binop) (v1 v2 : val Ti) : Prop :=
+    match v1, v2 with
+    | VBase vb1, VBase vb2 => base_val_binop_ok Γ Γm op vb1 vb2 | _, _ => False
+    end.
+  Global Arguments val_binop_ok _ _ !_ !_ !_ /.
+  Definition val_binop (Γ : env Ti) (op : binop) (v1 v2 : val Ti) : val Ti :=
+    match v1, v2 with
+    | VBase vb1, VBase vb2 => VBase (base_val_binop Γ op vb1 vb2) | _, _ => v1
+    end.
+  Global Arguments val_binop _ !_ !_ !_ /.
+
+  Inductive cast_typed (Γ : env Ti) : type Ti → type Ti → Prop :=
+    | cast_typed_self τ : cast_typed Γ τ τ
+    | TBase_cast_typed τb1 τb2 :
+       base_cast_typed Γ τb1 τb2 → cast_typed Γ (baseT τb1) (baseT τb2)
+    | TBase_TVoid_cast_typed τ : cast_typed Γ τ voidT.
+  Definition val_cast_ok (Γ : env Ti) (Γm : memenv Ti)
+      (τ : type Ti) (v : val Ti) : Prop :=
+    match v, τ with
+    | VBase vb, baseT τb => base_val_cast_ok Γ Γm τb vb | _, _ => True
+    end.
+  Global Arguments val_cast_ok _ _ !_ !_ /.
+  Definition val_cast (τ : type Ti) (v : val Ti) : val Ti :=
+    match v, τ with
+    | VBase vb, baseT τb => VBase (base_val_cast τb vb)
+    | _, voidT => VBase VVoid | _ , _ => v
+    end.
+  Global Arguments val_cast !_ !_ /.
+End operations.
+
+Section properties.
+Context `{EnvSpec Ti}.
+Implicit Types Γ : env Ti.
+Implicit Types Γm : memenv Ti.
+Implicit Types τb σb : base_type Ti.
+Implicit Types τ σ : type Ti.
+Implicit Types a : addr Ti.
+Implicit Types vb : base_val Ti.
+Implicit Types v : val Ti.
+Implicit Types m : mem Ti.
+
+(** ** Properties of operations on addresses *)
+Lemma addr_plus_typed Γ Γm a σ j :
+  ✓ Γ → (Γ,Γm) ⊢ a : σ → addr_plus_ok Γ Γm j a → (Γ,Γm) ⊢ addr_plus Γ j a : σ.
+Proof.
+  intros ? [o r i τ σ' σc ??????] (?&?&?);
+    constructor; simpl in *; split_ands; auto.
+  { apply Nat2Z.inj_le. by rewrite Nat2Z.inj_mul, Z2Nat.id by done. }
+  apply Nat2Z.inj. rewrite Z2Nat_inj_mod, Z2Nat.id by done.
+  rewrite Z.mod_add, <-Z2Nat_inj_mod; auto with f_equal.
+  rewrite (Nat2Z.inj_iff _ 0); eauto using size_of_ne_0,
+    ref_typed_type_valid, castable_type_valid.
+Qed.
+Lemma addr_plus_ok_weaken Γ1 Γ2 Γm1 Γm2 a σ j :
+  ✓ Γ1 → (Γ1,Γm1) ⊢ a : σ → addr_plus_ok Γ1 Γm1 j a →
+  Γ1 ⊆ Γ2 → (∀ o, index_alive Γm1 o → index_alive Γm2 o) →
+  addr_plus_ok Γ2 Γm2 j a.
+Proof.
+  unfold addr_plus_ok. intros ?? (?&?&?) ??. erewrite <-addr_size_of_weaken,
+    <-(size_of_weaken _ Γ2) by eauto using addr_typed_type_base_valid; eauto.
+Qed.
+Lemma addr_plus_weaken Γ1 Γ2 Γm1 a σ j :
+  ✓ Γ1 → (Γ1,Γm1) ⊢ a : σ → Γ1 ⊆ Γ2 → addr_plus Γ1 j a = addr_plus Γ2 j a.
+Proof.
+  intros ? [o r i τ σ' σc'] ?; simpl. by erewrite size_of_weaken
+    by eauto using ref_typed_type_valid, castable_type_valid.
+Qed.
+Lemma addr_type_plus Γ a j : type_of (addr_plus Γ j a) = type_of a.
+Proof. by destruct a. Qed.
+Lemma addr_type_base_plus Γ a j :
+  addr_type_base (addr_plus Γ j a) = addr_type_base a.
+Proof. by destruct a. Qed.
+Lemma addr_index_plus Γ a j : addr_index (addr_plus Γ j a) = addr_index a.
+Proof. by destruct a. Qed.
+Lemma addr_plus_0 Γ a : addr_plus Γ 0 a = a.
+Proof. destruct a; simpl. by rewrite Z.mul_0_l, Z.add_0_r, Nat2Z.id. Qed.
+Lemma addr_plus_plus Γ a j1 j2 :
+  (0 ≤ addr_byte a + j2 * size_of' Γ a)%Z →
+  addr_plus Γ j1 (addr_plus Γ j2 a) = addr_plus Γ (j1 + j2) a.
+Proof.
+  intros. destruct a as [o r i σ σc]; do 2 f_equal'.
+  by rewrite Z2Nat.id, (Z.add_comm j1), Z.mul_add_distr_r, Z.add_assoc.
+Qed.
+Lemma addr_plus_plus_nat Γ a (j1 j2 : nat) :
+  addr_plus Γ j1 (addr_plus Γ j2 a) = addr_plus Γ(j1 + j2)%nat a.
+Proof. rewrite Nat2Z.inj_add. apply addr_plus_plus; auto with zpos. Qed.
+Lemma addr_is_obj_plus Γ a j : addr_is_obj (addr_plus Γ j a) ↔ addr_is_obj a.
+Proof. by destruct a. Qed.
+Lemma addr_ref_base_plus Γ a j :
+  addr_ref_base (addr_plus Γ j a) = addr_ref_base a.
+Proof. by destruct a. Qed.
+Lemma addr_byte_representable Γ Γm a σ :
+  ✓ Γ → (Γ,Γm) ⊢ a : σ → int_typed (addr_byte a) sptrT.
+Proof.
+  destruct 2 as [o r i τ σ σc ?? [_ ?]]; simpl; split.
+  { transitivity 0; auto using int_lower_nonpos with zpos. }
+  assert (size_of Γ σ * ref_size r ≤ size_of Γ τ) by eauto using size_of_ref.
+  lia.
+Qed.
+Lemma addr_minus_typed Γ Γm a1 a2 σ :
+  ✓ Γ → (Γ,Γm) ⊢ a1 : σ → (Γ,Γm) ⊢ a2 : σ →
+  int_typed (addr_minus Γ a1 a2) sptrT.
+Proof.
+  intros HΓ Ha1 Ha2; unfold addr_minus; simplify_type_equality'.
+  assert (0 < size_of Γ σ)%Z.
+  { apply (Nat2Z.inj_lt 0); eauto using size_of_pos, addr_typed_type_valid. }
+  assert (int_upper sptrT ≤ size_of Γ σ * int_upper sptrT)%Z.
+  { transitivity (1 * int_upper sptrT)%Z; [lia|].
+    apply Z.mul_le_mono_nonneg_r; auto using int_upper_pos with zpos. }
+  destruct (addr_byte_representable Γ Γm a1 σ) as [_ ?]; auto.
+  destruct (addr_byte_representable Γ Γm a2 σ) as [_ ?]; auto.
+  split; [|apply Z.div_lt_upper_bound; lia].
+  apply Z.div_le_lower_bound; auto. rewrite int_lower_upper_signed by done; lia.
+Qed.
+Lemma addr_minus_ok_weaken Γm1 Γm2 a1 a2:
+  addr_minus_ok Γm1 a1 a2 → (∀ o, index_alive Γm1 o → index_alive Γm2 o) →
+  addr_minus_ok Γm2 a1 a2.
+Proof. intros [??]; split; eauto. Qed.
+Lemma addr_minus_weaken Γ1 Γ2 mm1 a1 a2 σ1 :
+  ✓ Γ1 → (Γ1,mm1) ⊢ a1 : σ1 →
+  Γ1 ⊆ Γ2 → addr_minus Γ1 a1 a2 = addr_minus Γ2 a1 a2.
+Proof.
+  intros. unfold addr_minus; simplify_type_equality.
+  by erewrite (size_of_weaken Γ1 Γ2) by eauto using addr_typed_type_valid.
+Qed.
+Lemma addr_cast_typed Γ Γm a σ σc :
+  (Γ,Γm) ⊢ a : σ → addr_cast_ok Γ Γm σc a → (Γ,Γm) ⊢ addr_cast σc a : σc.
+Proof. intros [] (?&?&?); constructor; naive_solver. Qed.
+Lemma addr_cast_ok_weaken Γ1 Γ2 Γm1 Γm2 a σ σc :
+  ✓ Γ1 → (Γ1,Γm1) ⊢ a : σ → (∀ o, index_alive Γm1 o → index_alive Γm2 o) →
+  addr_cast_ok Γ1 Γm1 σc a → Γ1 ⊆ Γ2 → addr_cast_ok Γ2 Γm2 σc a.
+Proof.
+  intros ??? (?&?&?); repeat split; auto. by erewrite <-size_of_weaken
+    by eauto using castable_type_valid, addr_typed_type_base_valid.
+Qed.
+Lemma addr_type_cast a σc : type_of (addr_cast σc a) = σc.
+Proof. by destruct a. Qed.
+Lemma addr_index_cast a σc : addr_index (addr_cast σc a) = addr_index a.
+Proof. by destruct a. Qed.
+Lemma addr_ref_cast Γ a σc : addr_ref Γ (addr_cast σc a) = addr_ref Γ a.
+Proof. by destruct a. Qed.
+Lemma addr_ref_byte_cast Γ a σc :
+  addr_ref_byte Γ (addr_cast σc a) = addr_ref_byte Γ a.
+Proof. by destruct a. Qed.
+Lemma addr_cast_self Γ Γm a σ : (Γ,Γm) ⊢ a : σ → addr_cast σ a = a.
+Proof. by destruct 1. Qed.
+Lemma addr_is_obj_cast a σc :
+  addr_is_obj (addr_cast σc a) ↔ σc = addr_type_base a.
+Proof. by destruct a. Qed.
+Lemma addr_ref_plus_char_cast Γ Γm a σ j :
+  ✓ Γ → (Γ,Γm) ⊢ a : σ → addr_is_obj a → j < size_of Γ σ →
+  addr_ref Γ (addr_plus Γ j (addr_cast ucharT a)) = addr_ref Γ a.
+Proof.
+  destruct 2 as [o r i τ σ σc ?????]; intros ??; simplify_equality'; f_equal.
+  rewrite size_of_uchar, Z.mul_1_r,Z2Nat.inj_add, !Nat2Z.id by auto with zpos.
+  symmetry. apply Nat.div_unique with (i `mod` size_of Γ σ + j); [lia|].
+  by rewrite Nat.add_assoc, <-Nat.div_mod
+    by eauto using ref_typed_type_valid, size_of_ne_0.
+Qed.
+Lemma addr_ref_byte_plus_char_cast Γ Γm a σ j :
+  ✓ Γ → (Γ,Γm) ⊢ a : σ → addr_is_obj a → j < size_of Γ σ →
+  addr_ref_byte Γ (addr_plus Γ j (addr_cast ucharT a)) = j.
+Proof.
+  destruct 2 as [o r i τ σ σc ?????? Hiσ]; intros; simplify_equality'.
+  f_equal. rewrite size_of_uchar.
+  rewrite Z.mul_1_r, Z2Nat.inj_add, !Nat2Z.id by auto with zpos.
+  rewrite <-Nat.add_mod_idemp_l
+    by eauto using ref_typed_type_valid, size_of_ne_0.
+  rewrite Hiσ, Nat.add_0_l. by apply Nat.mod_small.
+Qed.
+Lemma addr_byte_lt_size_char_cast Γ Γm a σ j :
+  ✓ Γ → (Γ,Γm) ⊢ a : σ → addr_is_obj a → j < size_of Γ σ →
+  addr_byte a < size_of Γ (addr_type_base a) * ref_size (addr_ref_base a) →
+  addr_byte (addr_plus Γ j (addr_cast ucharT a))
+    < size_of Γ (addr_type_base a) * ref_size (addr_ref_base a).
+Proof.
+  destruct 2 as [o r i τ σ σc ?????? Hiσ]; intros; simplify_equality'.
+  rewrite size_of_uchar, Z.mul_1_r,Z2Nat.inj_add, !Nat2Z.id by auto with zpos.
+  apply Nat.lt_le_trans with (i + size_of Γ σ); [lia|].
+  apply Nat.div_exact in Hiσ; eauto using ref_typed_type_valid, size_of_ne_0.
+  rewrite Hiσ, <-Nat.mul_succ_r. apply Nat.mul_le_mono_l, Nat.le_succ_l.
+  apply Nat.div_lt_upper_bound;
+    eauto using ref_typed_type_valid, size_of_ne_0.
+Qed.
+Lemma addr_elt_typed Γ Γm a rs σ σ' :
+  ✓ Γ → (Γ,Γm) ⊢ a : σ → addr_strict Γ a → Γ ⊢ rs : σ ↣ σ' →
+  ref_seg_offset rs = 0 → (Γ,Γm) ⊢ addr_elt Γ rs a : σ'.
+Proof.
+  rewrite addr_typed_alt. intros ? (?&?&?&?&?&?&?&Hcast&?) ? Hrs ?.
+  destruct a as [o r i τ σ'' σc]; simplify_equality'.
+  apply castable_alt in Hcast; destruct Hcast as [?|[?|?]];
+    simplify_equality'; try solve [inversion Hrs].
+  erewrite path_type_check_complete by eauto; simpl; constructor; auto.
+  * apply ref_typed_cons; exists σ; split; auto.
+    apply ref_set_offset_typed; auto.
+    apply Nat.div_lt_upper_bound; eauto using size_of_ne_0,ref_typed_type_valid.
+  * lia.
+  * by rewrite Nat.mod_0_l by eauto using size_of_ne_0, ref_typed_type_valid,
+      ref_seg_typed_type_valid, castable_type_valid.
+Qed.
+Lemma addr_elt_strict Γ Γm a rs σ σ' :
+  ✓ Γ → (Γ,Γm) ⊢ a : σ → Γ ⊢ rs : σ ↣ σ' → addr_strict Γ (addr_elt Γ rs a).
+Proof.
+  rewrite addr_typed_alt. intros ? (?&?&?&?&?&?&?&Hcast&?) Hrs.
+  destruct a as [o r i τ σ'' σc]; simplify_equality'.
+  erewrite path_type_check_complete by eauto; simpl.
+  apply Nat.mul_pos_pos.
+  * eauto using size_of_pos, ref_typed_type_valid,
+      ref_seg_typed_type_valid, castable_type_valid.
+  * destruct Hrs; simpl; lia.
+Qed.
+Lemma addr_elt_weaken Γ1 Γ2 Γm1 a rs σ σ' :
+  ✓ Γ1 → (Γ1,Γm1) ⊢ a : σ → Γ1 ⊢ rs : σ ↣ σ' → Γ1 ⊆ Γ2 →
+  addr_elt Γ1 rs a = addr_elt Γ2 rs a.
+Proof.
+  intros. unfold addr_elt; simplify_type_equality.
+  by erewrite addr_ref_weaken, !path_type_check_complete
+    by eauto using ref_seg_typed_weaken.
+Qed.
+Lemma addr_plus_ok_refine Γ f Γm1 Γm2 a1 a2 σ j :
+  a1 ⊑{Γ,f@Γm1↦Γm2} a2 : σ → addr_plus_ok Γ Γm1 j a1 → addr_plus_ok Γ Γm2 j a2.
+Proof.
+  unfold addr_plus_ok. intros Ha (?&?&?).
+  destruct (addr_byte_refine_help Γ f Γm1 Γm2 a1 a2 σ) as (i&?&?); auto.
+  destruct Ha as [??????????? (?&?&?&?)]; simplify_equality'; split; eauto; lia.
+Qed.
+Lemma addr_plus_refine Γ f Γm1 Γm2 a1 a2 σ j :
+  ✓ Γ → addr_plus_ok Γ Γm1 j a1 →
+  a1 ⊑{Γ,f@Γm1↦Γm2} a2 : σ → addr_plus Γ j a1 ⊑{Γ,f@Γm1↦Γm2} addr_plus Γ j a2 : σ.
+Proof.
+  intros ? Ha' Ha. destruct Ha' as (_&?&?), Ha as
+    [o o' r r' r'' i i'' τ τ' σ σc ??????????? Hr'']; simplify_equality'.
+  econstructor; eauto.
+  { apply Nat2Z.inj_le. by rewrite Nat2Z.inj_mul, Z2Nat.id by done. }
+  { apply Nat2Z.inj. rewrite Z2Nat_inj_mod, Z2Nat.id by done.
+    rewrite Z.mod_add, <-Z2Nat_inj_mod; auto with f_equal.
+    rewrite (Nat2Z.inj_iff _ 0).
+    eauto using size_of_ne_0, ref_typed_type_valid, castable_type_valid. }
+  destruct Hr'' as [i|r i]; simplify_equality'; [|by constructor].
+  apply ref_refine_nil_alt; auto. rewrite ref_offset_freeze.
+  rewrite Nat2Z.inj_add, Nat2Z.inj_mul. 
+  transitivity (Z.to_nat ((i + j * size_of Γ σc) +
+    size_of Γ σ * ref_offset r')); [f_equal; lia |].
+  by rewrite Z2Nat.inj_add, Z2Nat.inj_mul, !Nat2Z.id
+    by auto using Z.mul_nonneg_nonneg with lia.
+Qed.
+Lemma addr_minus_ok_refine Γ f Γm1 Γm2 a1 a2 a3 a4 σ :
+  a1 ⊑{Γ,f@Γm1↦Γm2} a2 : σ → a3 ⊑{Γ,f@Γm1↦Γm2} a4 : σ →
+  addr_minus_ok Γm1 a1 a3 → addr_minus_ok Γm2 a2 a4.
+Proof.
+  destruct 1 as [??????????? (?&?&?&?) ?????????? []],
+    1 as [??????????? (?&?&?&?) ?????????? []];
+    intros (?&?&Hr); simplify_equality'; eauto.
+  rewrite !fmap_app, !ref_freeze_freeze by eauto; eauto with congruence.
+Qed.
+Lemma addr_minus_refine Γ f Γm1 Γm2 a1 a2 a3 a4 σ :
+  addr_minus_ok Γm1 a1 a3 → a1 ⊑{Γ,f@Γm1↦Γm2} a2 : σ →
+  a3 ⊑{Γ,f@Γm1↦Γm2} a4 : σ → addr_minus Γ a1 a3 = addr_minus Γ a2 a4.
+Proof.
+  intros (?&?&?).
+  destruct 1 as [o1 o2 r1 r2 r3 i1 i3 τ1 τ2 σ1 σc ??????????? Hr3],
+    1 as [o4 o5 r4 r5 r6 i4 i6 τ4 τ5 σ3 σc4 ??????????? Hr6].
+  destruct Hr3, Hr6; simplify_type_equality'; f_equal; lia.
+Qed.
+Lemma addr_cast_ok_refine Γ f Γm1 Γm2 a1 a2 σ σc :
+  ✓ Γ → a1 ⊑{Γ,f@Γm1↦Γm2} a2 : σ →
+  addr_cast_ok Γ Γm1 σc a1 → addr_cast_ok Γ Γm2 σc a2.
+Proof.
+  destruct 2 as [o o' r r' r'' i i'' τ τ' σ σc' (?&?&?&?) ?????????? []];
+    intros (?&?&?); simplify_equality'; split_ands; eauto.
+  destruct (castable_divide Γ σ σc) as [z ->]; auto. rewrite ref_offset_freeze.
+  destruct (decide (size_of Γ σc = 0)) as [->|?]; [done|].
+  by rewrite !(Nat.mul_comm (_ * size_of _ _)), Nat.mul_assoc, Nat.mod_add.
+Qed.
+Lemma addr_cast_refine Γ f Γm1 Γm2 a1 a2 σ σc :
+  addr_cast_ok Γ Γm1 σc a1 → a1 ⊑{Γ,f@Γm1↦Γm2} a2 : σ →
+  addr_cast σc a1 ⊑{Γ,f@Γm1↦Γm2} addr_cast σc a2 : σc.
+Proof. intros (?&?&?). destruct 1; simplify_equality'; econstructor; eauto. Qed.
+Lemma addr_elt_refine Γ f Γm1 Γm2 a1 a2 rs σ σ' :
+  ✓ Γ → a1 ⊑{Γ,f@Γm1↦Γm2} a2 : σ → addr_strict Γ a1 → Γ ⊢ rs : σ ↣ σ' →
+  ref_seg_offset rs = 0 → addr_elt Γ rs a1 ⊑{Γ,f@Γm1↦Γm2} addr_elt Γ rs a2 : σ'.
+Proof.
+  intros ? [o o' r r' r'' i i'' τ τ' σ'' ??????????? Hcst Hr''] ? Hrs ?; simpl.
+  apply castable_alt in Hcst; destruct Hcst as [<-|[?|?]];
+    simplify_equality'; try solve [inversion Hrs].
+  erewrite path_type_check_complete by eauto; simpl. econstructor; eauto.
+  * apply ref_typed_cons; exists σ''; split; auto.
+    apply ref_set_offset_typed; auto.
+    apply Nat.div_lt_upper_bound; eauto using size_of_ne_0,ref_typed_type_valid.
+  * lia.
+  * by rewrite Nat.mod_0_l by eauto using size_of_ne_0, ref_typed_type_valid,
+      ref_seg_typed_type_valid, castable_type_valid.
+  * destruct Hr'' as [i''|]; simplify_equality'; [|by constructor].
+    apply ref_refine_ne_nil_alt.
+    by rewrite ref_set_offset_set_offset, (Nat.mul_comm (size_of _ _)),
+      Nat.div_add, Nat.div_small, Nat.add_0_l, ref_set_offset_offset by lia.
+Qed.
+
+(** ** Properties of operations on pointers *)
+Global Instance ptr_compare_ok_dec Γm c p1 p2 :
+  Decision (ptr_compare_ok Γm c p1 p2).
+Proof. destruct p1, p2, c; apply _. Defined.
+Global Instance ptr_plus_ok_dec Γ Γm j p : Decision (ptr_plus_ok Γ Γm j p).
+Proof. destruct p; apply _. Defined.
+Global Instance ptr_minus_ok_dec Γm p1 p2 : Decision (ptr_minus_ok Γm p1 p2).
+Proof. destruct p1, p2; apply _. Defined.
+Global Instance ptr_cast_ok_dec Γ Γm σc p : Decision (ptr_cast_ok Γ Γm σc p).
+Proof. destruct p; apply _. Defined.
+Lemma ptr_plus_typed Γ Γm p σ j :
+  ✓ Γ → (Γ,Γm) ⊢ p : σ → ptr_plus_ok Γ Γm j p → (Γ,Γm) ⊢ ptr_plus Γ j p : σ.
+Proof. destruct 2; simpl; constructor; eauto using addr_plus_typed. Qed.
+Lemma ptr_minus_typed Γ Γm p1 p2 σ :
+  ✓ Γ → (Γ,Γm) ⊢ p1 : σ → (Γ,Γm) ⊢ p2 : σ →
+  int_typed (ptr_minus Γ p1 p2) sptrT.
+Proof.
+  destruct 2, 1; simpl;
+    eauto using addr_minus_typed, int_typed_small with lia.
+Qed.
+Lemma ptr_cast_typed Γ Γm p σ σc :
+  (Γ,Γm) ⊢ p : σ → ptr_cast_ok Γ Γm σc p →
+  ptr_type_valid Γ σc → (Γ,Γm) ⊢ ptr_cast σc p : σc.
+Proof. destruct 1; simpl; constructor; eauto using addr_cast_typed. Qed.
+
+Lemma ptr_compare_ok_weaken Γm1 Γm2 c p1 p2 :
+  ptr_compare_ok Γm1 c p1 p2 → (∀ o, index_alive Γm1 o → index_alive Γm2 o) →
+  ptr_compare_ok Γm2 c p1 p2.
+Proof. destruct p1, p2, c; simpl; eauto using addr_minus_ok_weaken. Qed.
+Lemma ptr_compare_weaken Γ1 Γ2 Γm1 c p1 p2 τ1 τ2 :
+  ✓ Γ1 → (Γ1,Γm1) ⊢ p1 : τ1 → (Γ1,Γm1) ⊢ p2 : τ2 →
+  Γ1 ⊆ Γ2 → ptr_compare Γ1 c p1 p2 = ptr_compare Γ2 c p1 p2.
+Proof.
+  destruct 2,1,c; simpl; intros; done || by erewrite addr_minus_weaken by eauto.
+Qed.
+Lemma ptr_plus_ok_weaken Γ1 Γ2 Γm1 Γm2 p τ j :
+  ✓ Γ1 → (Γ1,Γm1) ⊢ p : τ → ptr_plus_ok Γ1 Γm1 j p →
+  Γ1 ⊆ Γ2 → (∀ o, index_alive Γm1 o → index_alive Γm2 o) →
+  ptr_plus_ok Γ2 Γm2 j p.
+Proof. destruct 2; simpl; eauto using addr_plus_ok_weaken. Qed.
+Lemma ptr_plus_weaken Γ1 Γ2 Γm1 p τ j :
+  ✓ Γ1 → (Γ1,Γm1) ⊢ p : τ → Γ1 ⊆ Γ2 → ptr_plus Γ1 j p = ptr_plus Γ2 j p.
+Proof. destruct 2; simpl; eauto using addr_plus_weaken, f_equal. Qed.
+Lemma ptr_minus_ok_weaken Γm1 Γm2 p1 p2:
+  ptr_minus_ok Γm1 p1 p2 → (∀ o, index_alive Γm1 o → index_alive Γm2 o) →
+  ptr_minus_ok Γm2 p1 p2.
+Proof. destruct p1, p2; simpl; eauto using addr_minus_ok_weaken. Qed.
+Lemma ptr_minus_weaken Γ1 Γ2 Γm1 p1 p2 τ1 τ2 :
+  ✓ Γ1 → (Γ1,Γm1) ⊢ p1 : τ1 → (Γ1,Γm1) ⊢ p2 : τ2 →
+  Γ1 ⊆ Γ2 → ptr_minus Γ1 p1 p2 = ptr_minus Γ2 p1 p2.
+Proof. destruct 2, 1; simpl; eauto using addr_minus_weaken. Qed.
+Lemma ptr_cast_ok_weaken Γ1 Γ2 Γm1 Γm2 p τ σc :
+  ✓ Γ1 → (Γ1,Γm1) ⊢ p : τ → ptr_cast_ok Γ1 Γm1 σc p → Γ1 ⊆ Γ2 →
+  (∀ o, index_alive Γm1 o → index_alive Γm2 o) → ptr_cast_ok Γ2 Γm2 σc p.
+Proof. destruct 2; simpl; eauto using addr_cast_ok_weaken. Qed.
+Lemma ptr_compare_ok_alive_l Γm c p1 p2 :
+  ptr_compare_ok Γm c p1 p2 → ptr_alive Γm p1.
+Proof. destruct p1, p2, c; try done; by intros [??]. Qed.
+Lemma ptr_compare_ok_alive_r Γm c p1 p2 :
+  ptr_compare_ok Γm c p1 p2 → ptr_alive Γm p2.
+Proof. destruct p1, p2, c; done || intros (?&?&?); simpl in *; congruence. Qed.
+Lemma ptr_plus_ok_alive Γ Γm p j : ptr_plus_ok Γ Γm j p → ptr_alive Γm p.
+Proof. destruct p. done. by intros [??]. Qed.
+Lemma ptr_minus_ok_alive_l Γm p1 p2 : ptr_minus_ok Γm p1 p2 → ptr_alive Γm p1.
+Proof. destruct p1, p2; try done. by intros [??]. Qed.
+Lemma ptr_minus_ok_alive_r Γm p1 p2 : ptr_minus_ok Γm p1 p2 → ptr_alive Γm p2.
+Proof. destruct p1, p2; try done. intros (?&?&?); simpl in *; congruence. Qed.
+Lemma ptr_cast_ok_alive Γ Γm p σ : ptr_cast_ok Γ Γm σ p → ptr_alive Γm p.
+Proof. destruct p. done. by intros [??]. Qed.
+
+Lemma ptr_compare_ok_refine Γ Γm1 Γm2 f c p1 p2 p3 p4 σ :
+  p1 ⊑{Γ,f@Γm1↦Γm2} p2 : σ → p3 ⊑{Γ,f@Γm1↦Γm2} p4 : σ →
+  ptr_compare_ok Γm1 c p1 p3 → ptr_compare_ok Γm2 c p2 p4.
+Proof.
+  destruct 1, 1, c; simpl; eauto using addr_minus_ok_refine, addr_alive_refine.
+Qed.
+Lemma ptr_compare_refine Γ f Γm1 Γm2 c p1 p2 p3 p4 σ :
+  ✓ Γ → ptr_compare_ok Γm1 c p1 p3 →
+  p1 ⊑{Γ,f@Γm1↦Γm2} p2 : σ → p3 ⊑{Γ,f@Γm1↦Γm2} p4 : σ →
+  ptr_compare Γ c p1 p3 = ptr_compare Γ c p2 p4.
+Proof.
+  destruct 3, 1, c; simpl; done || by erewrite addr_minus_refine by eauto.
+Qed.
+Lemma ptr_plus_ok_refine Γ Γm1 Γm2 f p1 p2 σ j :
+  p1 ⊑{Γ,f@Γm1↦Γm2} p2 : σ → ptr_plus_ok Γ Γm1 j p1 → ptr_plus_ok Γ Γm2 j p2.
+Proof. destruct 1; simpl; eauto using addr_plus_ok_refine. Qed.
+Lemma ptr_plus_refine Γ f Γm1 Γm2 p1 p2 σ j :
+  ✓ Γ → ptr_plus_ok Γ Γm1 j p1 →
+  p1 ⊑{Γ,f@Γm1↦Γm2} p2 : σ → ptr_plus Γ j p1 ⊑{Γ,f@Γm1↦Γm2} ptr_plus Γ j p2 : σ.
+Proof. destruct 3; simpl; constructor; eauto using addr_plus_refine. Qed.
+Lemma ptr_minus_ok_refine Γ Γm1 Γm2 f p1 p2 p3 p4 σ :
+  p1 ⊑{Γ,f@Γm1↦Γm2} p2 : σ → p3 ⊑{Γ,f@Γm1↦Γm2} p4 : σ →
+  ptr_minus_ok Γm1 p1 p3 → ptr_minus_ok Γm2 p2 p4.
+Proof. destruct 1, 1; simpl; eauto using addr_minus_ok_refine. Qed.
+Lemma ptr_minus_refine Γ f Γm1 Γm2 p1 p2 p3 p4 σ :
+  ✓ Γ → ptr_minus_ok Γm1 p1 p3 →
+  p1 ⊑{Γ,f@Γm1↦Γm2} p2 : σ → p3 ⊑{Γ,f@Γm1↦Γm2} p4 : σ →
+  ptr_minus Γ p1 p3 = ptr_minus Γ p2 p4.
+Proof. destruct 3, 1; simpl; eauto using addr_minus_refine. Qed.
+Lemma ptr_cast_ok_refine Γ f Γm1 Γm2 p1 p2 σ σc :
+  ✓ Γ → p1 ⊑{Γ,f@Γm1↦Γm2} p2 : σ →
+  ptr_cast_ok Γ Γm1 σc p1 → ptr_cast_ok Γ Γm2 σc p2.
+Proof. destruct 2; simpl; eauto using addr_cast_ok_refine. Qed.
+Lemma ptr_cast_refine Γ f Γm1 Γm2 p1 p2 σ σc :
+  ptr_cast_ok Γ Γm1 σc p1 → ptr_type_valid Γ σc → p1 ⊑{Γ,f@Γm1↦Γm2} p2 : σ →
+  ptr_cast σc p1 ⊑{Γ,f@Γm1↦Γm2} ptr_cast σc p2 : σc.
+Proof. destruct 3; constructor; eauto using addr_cast_refine. Qed.
+
+(** ** Properties of operations on base values *)
+Definition base_val_true_false_dec Γm vb :
+  { base_val_true Γm vb ∧ ¬base_val_false vb }
+  + { ¬base_val_true Γm vb ∧ base_val_false vb }
+  + { ¬base_val_true Γm vb ∧ ¬base_val_false vb }.
+Proof.
+ refine
+  match vb with
+  | VInt _ x => inleft (cast_if_not (decide (x = 0)))
+  | VPtr (Ptr a) =>
+    if decide (index_alive Γm (addr_index a))
+    then inleft (left _) else inright _
+  | VPtr (NULL _) => inleft (right _)
+  | _ => inright _
+  end; abstract naive_solver.
+Defined.
+Lemma base_val_true_weaken Γ Γm1 Γm2 vb :
+  base_val_true Γm1 vb → (∀ o, index_alive Γm1 o → index_alive Γm2 o) →
+  base_val_true Γm2 vb.
+Proof. destruct vb as [| | |[]|]; simpl; auto. Qed.
+Global Instance base_val_unop_ok_dec Γm op vb :
+  Decision (base_val_unop_ok Γm op vb).
+Proof. destruct vb, op; try apply _. Defined.
+Global Instance base_val_binop_ok_dec Γ Γm op vb1 vb2 :
+  Decision (base_val_binop_ok Γ Γm op vb1 vb2).
+Proof.
+  destruct vb1, vb2, op as [|op| |]; try apply _; destruct op; apply _.
+Defined.
+Global Instance base_val_cast_ok_dec Γ Γm σb vb :
+  Decision (base_val_cast_ok Γ Γm σb vb).
+Proof. destruct vb, σb; apply _. Defined.
+Lemma base_unop_typed_type_valid Γ op τb σb :
+  base_unop_typed op τb σb → ✓{Γ} τb → ✓{Γ} σb.
+Proof. destruct 1; constructor. Qed.
+Lemma base_binop_typed_type_valid Γ op τb1 τb2 σb :
+  base_binop_typed op τb1 τb2 σb → ✓{Γ} τb1 → ✓{Γ} τb2 → ✓{Γ} σb.
+Proof. destruct 1; constructor; eauto using TPtr_valid_inv. Qed.
+Lemma base_cast_typed_type_valid Γ τb σb :
+  base_cast_typed Γ τb σb → ✓{Γ} τb → ✓{Γ} σb.
+Proof. destruct 1; repeat constructor; eauto using TPtr_valid_inv. Qed.
+Lemma base_unop_type_of_sound op τb σb :
+  base_unop_type_of op τb = Some σb → base_unop_typed op τb σb.
+Proof. destruct τb, op; intros; simplify_option_equality; constructor. Qed.
+Lemma base_unop_type_of_complete op τb σb :
+  base_unop_typed op τb σb → base_unop_type_of op τb = Some σb.
+Proof. by destruct 1; simplify_option_equality. Qed.
+Lemma base_binop_type_of_sound op τb1 τb2 σb :
+  base_binop_type_of op τb1 τb2 = Some σb → base_binop_typed op τb1 τb2 σb.
+Proof.
+  destruct τb1, τb2, op; intros;
+    repeat (case_match || simplify_option_equality); constructor.
+Qed.
+Lemma base_binop_type_of_complete op τb1 τb2 σb :
+  base_binop_typed op τb1 τb2 σb → base_binop_type_of op τb1 τb2 = Some σb.
+Proof. by destruct 1; simplify_option_equality. Qed.
+Global Instance base_cast_typed_dec Γ τb σb: Decision (base_cast_typed Γ τb σb).
+Proof.
+ refine
+  match τb, σb with
+  | _, voidT => left _
+  | intT τi1, intT τi2 => left _
+  | τ1.*, τ2.* => cast_if (decide (τ1 = τ2 ∨ τ2 = voidT%T ∨ τ2 = ucharT%T ∨
+      τ1 = voidT%T ∧ ptr_type_valid Γ τ2 ∨ τ1 = ucharT%T ∧ ptr_type_valid Γ τ2))
+  | _, _ => right _
+  end%BT; abstract first
+    [by intuition; subst; constructor|by inversion 1; naive_solver].
+Defined.
+Lemma base_cast_typed_weaken Γ1 Γ2 τb σb :
+  base_cast_typed Γ1 τb σb → Γ1 ⊆ Γ2 → base_cast_typed Γ2 τb σb.
+Proof. destruct 1; constructor; eauto using ptr_type_valid_weaken. Qed.
+
+Lemma base_val_0_typed Γ Γm τb : ✓{Γ} τb → (Γ,Γm) ⊢ base_val_0 τb : τb.
+Proof.
+  destruct 1; simpl; constructor. by apply int_typed_small. by constructor.
+Qed.
+Lemma base_val_unop_ok_weaken Γm1 Γm2 op vb :
+  base_val_unop_ok Γm1 op vb → (∀ o, index_alive Γm1 o → index_alive Γm2 o) →
+  base_val_unop_ok Γm2 op vb.
+Proof. destruct vb, op; simpl; eauto using ptr_alive_weaken. Qed.
+Lemma base_val_unop_typed Γ Γm op vb τb σb :
+  (Γ,Γm) ⊢ vb : τb → base_unop_typed op τb σb →
+  base_val_unop_ok Γm op vb → (Γ,Γm) ⊢ base_val_unop op vb : σb.
+Proof.
+  unfold base_val_unop_ok, base_val_unop. intros Hvτb Hσ Hop.
+  destruct Hσ as [τi|?|?|?]; inversion Hvτb; simplify_equality'; try done.
+  * typed_constructor. rewrite <-(idempotent (∪) (int_promote τi)).
+    apply int_arithop_typed; auto. by apply int_typed_small.
+  * typed_constructor. apply int_of_bits_typed.
+    by rewrite fmap_length, int_to_bits_length.
+  * typed_constructor. by apply int_typed_small; case_decide.
+  * typed_constructor. by apply int_typed_small; case_match.
+Qed.
+Lemma base_val_binop_ok_weaken Γ1 Γ2 Γm1 Γm2 op vb1 vb2 τb1 τb2 :
+  ✓ Γ1 → (Γ1,Γm1) ⊢ vb1 : τb1 → (Γ1,Γm1) ⊢ vb2 : τb2 →
+  base_val_binop_ok Γ1 Γm1 op vb1 vb2 → Γ1 ⊆ Γ2 →
+  (∀ o, index_alive Γm1 o → index_alive Γm2 o) →
+  base_val_binop_ok Γ2 Γm2 op vb1 vb2.
+Proof.
+  destruct 2, 1, op as [|[]| |]; simpl; auto; eauto 2 using
+    ptr_plus_ok_weaken, ptr_minus_ok_weaken, ptr_compare_ok_weaken.
+Qed.
+Lemma base_val_binop_weaken Γ1 Γ2 Γm1 op vb1 vb2 τb1 τb2 :
+  ✓ Γ1 → (Γ1,Γm1) ⊢ vb1 : τb1 → (Γ1,Γm1) ⊢ vb2 : τb2 → Γ1 ⊆ Γ2 →
+  base_val_binop Γ1 op vb1 vb2 = base_val_binop Γ2 op vb1 vb2.
+Proof.
+  destruct 2, 1, op as [|[]| |]; intros; f_equal';
+    eauto 2 using ptr_plus_weaken, ptr_minus_weaken.
+  by erewrite ptr_compare_weaken by eauto.
+Qed.
+Lemma base_val_binop_typed Γ Γm op vb1 vb2 τb1 τb2 σb :
+  ✓ Γ → (Γ,Γm) ⊢ vb1 : τb1 → (Γ,Γm) ⊢ vb2 : τb2 →
+  base_binop_typed op τb1 τb2 σb → base_val_binop_ok Γ Γm op vb1 vb2 →
+  (Γ,Γm) ⊢ base_val_binop Γ op vb1 vb2 : σb.
+Proof.
+  unfold base_val_binop_ok, base_val_binop. intros HΓ Hv1τb Hv2τb Hσ Hop.
+  revert Hv1τb Hv2τb.
+  destruct Hσ; inversion 1; inversion 1; simplify_equality'; try done.
+  * constructor. by case_match; apply int_typed_small.
+  * constructor. by apply int_arithop_typed.
+  * constructor. by apply int_shiftop_typed.
+  * constructor. apply int_of_bits_typed.
+    rewrite zip_with_length, !int_to_bits_length; lia.
+  * constructor. by case_match; apply int_typed_small.
+  * constructor. eapply ptr_plus_typed; eauto.
+  * constructor. eapply ptr_plus_typed; eauto.
+  * constructor. eapply ptr_plus_typed; eauto.
+  * constructor. eapply ptr_plus_typed; eauto.
+  * constructor. eapply ptr_minus_typed; eauto.
+Qed.
+Lemma base_cast_typed_self Γ τb : base_cast_typed Γ τb τb.
+Proof. destruct τb; constructor. Qed.
+Lemma base_val_cast_ok_weaken Γ1 Γ2 Γm1 Γm2 vb τb σb :
+  ✓ Γ1 → (Γ1,Γm1) ⊢ vb : τb → base_val_cast_ok Γ1 Γm1 σb vb →
+  Γ1 ⊆ Γ2 → (∀ o : index, index_alive Γm1 o → index_alive Γm2 o) →
+  base_val_cast_ok Γ2 Γm2 σb vb.
+Proof.
+  destruct 2, σb; simpl; eauto using ptr_cast_ok_weaken, ptr_alive_weaken.
+Qed.
+Lemma base_val_cast_typed Γ Γm vb τb σb :
+  ✓ Γ → (Γ,Γm) ⊢ vb : τb → base_cast_typed Γ τb σb →
+  base_val_cast_ok Γ Γm σb vb → (Γ,Γm) ⊢ base_val_cast σb vb : σb.
+Proof.
+  unfold base_val_cast_ok, base_val_cast. intros ? Hvτb Hσb Hok. revert Hvτb.
+  destruct Hσb; inversion 1; simplify_equality'; try (done || by constructor).
+  * intuition; simplify_equality. by constructor.
+  * constructor. by apply int_cast_typed.
+  * constructor. eapply ptr_cast_typed,
+      TPtr_valid_inv, base_val_typed_type_valid; eauto.
+  * constructor.
+    eapply ptr_cast_typed; eauto using TBase_ptr_valid, TVoid_valid.
+  * constructor. eapply ptr_cast_typed;
+      eauto using TBase_ptr_valid, TInt_valid.
+  * constructor. eapply ptr_cast_typed; eauto.
+  * constructor. eapply ptr_cast_typed; eauto.
+Qed.
+Lemma base_val_cast_ok_void Γ Γm vb :
+  (Γ,Γm) ⊢ vb : ucharT%BT → base_val_cast_ok Γ Γm voidT%BT vb.
+Proof. by inversion 1. Qed.
+Lemma base_val_cast_void vb : base_val_cast voidT vb = VVoid.
+Proof. by destruct vb. Qed.
+
+Lemma base_val_true_refine Γ f Γm1 Γm2 vb1 vb2 τb :
+  vb1 ⊑{Γ,f@Γm1↦Γm2} vb2 : τb → base_val_true Γm1 vb1 → base_val_true Γm2 vb2.
+Proof.
+   by destruct 1 as [| | |??? []|??? []| | |];
+     simpl; eauto using addr_alive_refine.
+Qed.
+Lemma base_val_false_refine Γ f Γm1 Γm2 vb1 vb2 τb :
+  vb1 ⊑{Γ,f@Γm1↦Γm2} vb2 : τb → base_val_false vb1 → base_val_false vb2.
+Proof. by destruct 1 as [| | |??? []|??? []| | |]. Qed.
+Lemma base_val_unop_ok_refine Γ f Γm1 Γm2 op vb1 vb2 τb :
+  vb1 ⊑{Γ,f@Γm1↦Γm2} vb2 : τb →
+  base_val_unop_ok Γm1 op vb1 → base_val_unop_ok Γm2 op vb2.
+Proof. by destruct op, 1; simpl; eauto using ptr_alive_refine. Qed.
+Lemma base_val_unop_refine Γ f Γm1 Γm2 op vb1 vb2 τb σb :
+  ✓ Γ → base_unop_typed op τb σb → base_val_unop_ok Γm1 op vb1 →
+  vb1 ⊑{Γ,f@Γm1↦Γm2} vb2 : τb →
+  base_val_unop op vb1 ⊑{Γ,f@Γm1↦Γm2} base_val_unop op vb2 : σb.
+Proof.
+  intros ? Hvτb ? Hvb. assert ((Γ,Γm2) ⊢ base_val_unop op vb2 : σb) as Hvb2.
+  { eauto using base_val_unop_typed,
+      base_val_refine_typed_r, base_val_unop_ok_refine. }
+  destruct Hvτb; inversion Hvb as [| | |p1 p2 ? Hp| | | |];
+    simplify_equality'; try done.
+  * refine_constructor. rewrite <-(idempotent (∪) (int_promote τi)).
+    apply int_arithop_typed; auto. by apply int_typed_small.
+  * refine_constructor. apply int_of_bits_typed.
+    by rewrite fmap_length, int_to_bits_length.
+  * refine_constructor. by apply int_typed_small; case_decide.
+  * destruct Hp; refine_constructor; by apply int_typed_small.
+Qed.
+Lemma base_val_binop_ok_refine Γ f Γm1 Γm2 op vb1 vb2 vb3 vb4 τb1 τb3 σb :
+  ✓ Γ → base_binop_typed op τb1 τb3 σb →
+  vb1 ⊑{Γ,f@Γm1↦Γm2} vb2 : τb1 → vb3 ⊑{Γ,f@Γm1↦Γm2} vb4 : τb3 →
+  base_val_binop_ok Γ Γm1 op vb1 vb3 → base_val_binop_ok Γ Γm2 op vb2 vb4.
+Proof.
+  intros ? Hσ. destruct 1, 1; try done; inversion Hσ;
+   try naive_solver eauto using ptr_minus_ok_alive_l, ptr_minus_ok_alive_r,
+    ptr_plus_ok_alive, ptr_plus_ok_refine, ptr_minus_ok_refine,
+    ptr_compare_ok_refine, ptr_compare_ok_alive_l, ptr_compare_ok_alive_r.
+Qed.
+Lemma base_val_binop_refine Γ f Γm1 Γm2 op vb1 vb2 vb3 vb4 τb1 τb3 σb :
+  ✓ Γ → base_binop_typed op τb1 τb3 σb → base_val_binop_ok Γ Γm1 op vb1 vb3 →
+  vb1 ⊑{Γ,f@Γm1↦Γm2} vb2 : τb1 → vb3 ⊑{Γ,f@Γm1↦Γm2} vb4 : τb3 →
+  base_val_binop Γ op vb1 vb3 ⊑{Γ,f@Γm1↦Γm2} base_val_binop Γ op vb2 vb4 : σb.
+Proof.
+  intros ? Hσ ?; destruct 1, 1; try done; inversion Hσ; simplify_equality';
+    try first
+    [ by refine_constructor; eauto using int_arithop_typed,
+        int_arithop_typed, int_shiftop_typed, ptr_plus_refine
+    | exfalso; by eauto using ptr_minus_ok_alive_l, ptr_minus_ok_alive_r,
+        ptr_plus_ok_alive, ptr_compare_ok_alive_l, ptr_compare_ok_alive_r ].
+  * refine_constructor. by case_match; apply int_typed_small.
+  * refine_constructor. apply int_of_bits_typed.
+    rewrite zip_with_length, !int_to_bits_length; lia.
+  * erewrite ptr_compare_refine by eauto.
+    refine_constructor. by case_match; apply int_typed_small.
+  * erewrite ptr_minus_refine by eauto. refine_constructor.
+    eapply ptr_minus_typed; eauto using ptr_refine_typed_l, ptr_refine_typed_r.
+Qed.
+Lemma base_val_cast_ok_refine Γ f Γm1 Γm2 vb1 vb2 τb σb :
+  ✓ Γ → vb1 ⊑{Γ,f@Γm1↦Γm2} vb2 : τb →
+  base_val_cast_ok Γ Γm1 σb vb1 → base_val_cast_ok Γ Γm2 σb vb2.
+Proof.
+  assert (∀ vb, (Γ,Γm2) ⊢ vb : ucharT%BT → base_val_cast_ok Γ Γm2 ucharT vb).
+  { inversion 1; simpl; eauto using int_unsigned_pre_cast_ok,int_cast_ok_more. }
+  destruct σb, 2; simpl; try naive_solver eauto using
+    ptr_cast_ok_refine, ptr_cast_ok_alive, base_val_cast_ok_void,
+    int_unsigned_pre_cast_ok, int_cast_ok_more, ptr_alive_refine.
+Qed.
+Lemma base_val_cast_refine Γ f Γm1 Γm2 vb1 vb2 τb σb :
+  ✓ Γ → base_cast_typed Γ τb σb → base_val_cast_ok Γ Γm1 σb vb1 →
+  vb1 ⊑{Γ,f@Γm1↦Γm2} vb2 : τb →
+  base_val_cast σb vb1 ⊑{Γ,f@Γm1↦Γm2} base_val_cast σb vb2 : σb.
+Proof.
+  assert (∀ vb, (Γ,Γm2) ⊢ vb : ucharT%BT → base_val_cast ucharT vb = vb) as help.
+  { inversion 1; f_equal'. by rewrite int_cast_spec, int_typed_pre_cast
+      by eauto using int_unsigned_pre_cast_ok,int_cast_ok_more. }
+  destruct 2; inversion 2; simplify_equality';
+    intuition; simplify_equality'; try first
+    [ by exfalso; eauto using ptr_cast_ok_alive
+    | rewrite ?base_val_cast_void, ?help, ?int_cast_spec, ?int_typed_pre_cast
+        by eauto using int_unsigned_pre_cast_ok,int_cast_ok_more;
+      by refine_constructor; eauto using ptr_cast_refine, int_cast_typed,
+        ptr_cast_refine, TVoid_valid, TBase_ptr_valid, TInt_valid,
+        TPtr_valid_inv, base_val_typed_type_valid, base_val_refine_typed_l ].
+Qed.
+
+(** ** Properties of operations on values *)
+Lemma val_0_base Γ τb : val_0 Γ τb = VBase (base_val_0 τb).
+Proof. unfold val_0. by rewrite type_iter_base. Qed.
+Lemma val_0_array Γ τ n :
+  val_0 Γ (τ.[n]) = VArray τ (replicate n (val_0 Γ τ)).
+Proof. unfold val_0. by rewrite type_iter_array. Qed.
+Lemma val_0_compound Γ c s τs :
+  ✓ Γ → Γ !! s = Some τs → val_0 Γ (compoundT{c} s) =
+    match c with
+    | Struct_kind => VStruct s (val_0 Γ <$> τs)
+    | Union_kind => VUnion s 0 (default (VUnionAll s []) (τs !! 0) (val_0 Γ))
+    end.
+Proof.
+  intros HΓ Hs. unfold val_0; erewrite (type_iter_compound (=)); try done.
+  { by intros ????? ->. }
+  clear s τs Hs. intros ?? [] ? τs ?? Hgo; f_equal'; [|by destruct Hgo].
+  by apply Forall_fmap_ext.
+Qed.
+Lemma val_0_weaken Γ1 Γ2 τ :
+  ✓ Γ1 → ✓{Γ1} τ → Γ1 ⊆ Γ2 → val_0 Γ1 τ = val_0 Γ2 τ.
+Proof.
+  intros. apply (type_iter_weaken (=)); try done; [by intros ????? ->|].
+  intros ?? [] ? τs ?? Hgo; f_equal'; [|by destruct Hgo].
+  by apply Forall_fmap_ext.
+Qed.
+Lemma val_0_typed Γ Γm τ : ✓ Γ → ✓{Γ} τ → (Γ,Γm) ⊢ val_0 Γ τ : τ.
+Proof.
+  intros HΓ. revert τ. refine (type_env_ind _ HΓ _ _ _ _).
+  * intros τb. rewrite val_0_base.
+    typed_constructor; auto using base_val_0_typed.
+  * intros τ n ???. rewrite val_0_array.
+    typed_constructor; auto using replicate_length, Forall_replicate.
+  * intros [] s τs Hs _ IH ?; erewrite val_0_compound by eauto.
+    { typed_constructor; eauto. elim IH; csimpl; auto. }
+    by destruct IH; simplify_equality'; typed_constructor; eauto.
+Qed.
+Definition val_true_false_dec Γm v :
+  { val_true Γm v ∧ ¬val_false v } + { ¬val_true Γm v ∧ val_false v }
+  + { ¬val_true Γm v ∧ ¬val_false v }.
+Proof.
+ refine
+  match v with
+  | VBase vb =>
+     match base_val_true_false_dec Γm vb with
+     | inleft (left _) => inleft (left _)
+     | inleft (right _) => inleft (right _) | inright _ => inright _
+     end
+  | _ => inright _
+  end; abstract naive_solver.
+Defined.
+Lemma val_true_false Γm v : val_true Γm v → val_false v → False.
+Proof. by destruct (val_true_false_dec Γm v) as [[[??]|[??]]|[??]]. Qed.
+Lemma val_true_weaken Γ Γm1 Γm2 v :
+  val_true Γm1 v →
+  (∀ o, index_alive Γm1 o → index_alive Γm2 o) → val_true Γm2 v.
+Proof. destruct v; simpl; eauto using base_val_true_weaken. Qed.
+
+Global Instance val_unop_ok_dec Γm op v : Decision (val_unop_ok Γm op v).
+Proof. destruct v; try apply _. Defined.
+Global Instance val_binop_ok_dec Γ Γm op v1 v2 :
+  Decision (val_binop_ok Γ Γm op v1 v2).
+Proof. destruct v1, v2; apply _. Defined.
+Global Instance val_cast_ok_dec Γ Γm σ v : Decision (val_cast_ok Γ Γm σ v).
+Proof. destruct v, σ as [[]| |]; apply _. Defined.
+
+Lemma unop_typed_type_valid Γ op τ σ : unop_typed op τ σ → ✓{Γ} τ → ✓{Γ} σ.
+Proof.
+  destruct 1; eauto using TBase_valid,
+    TBase_valid_inv, base_unop_typed_type_valid.
+Qed.
+Lemma binop_typed_type_valid Γ op τ1 τ2 σ :
+  binop_typed op τ1 τ2 σ → ✓{Γ} τ1 → ✓{Γ} τ2 → ✓{Γ} σ.
+Proof.
+  destruct 1; eauto using TBase_valid,
+    TBase_valid_inv, base_binop_typed_type_valid.
+Qed.
+Lemma cast_typed_type_valid Γ τ σ : cast_typed Γ τ σ → ✓{Γ} τ → ✓{Γ} σ.
+Proof.
+  destruct 1; eauto using TBase_valid, TVoid_valid, TBase_valid,
+    TBase_valid_inv, base_cast_typed_type_valid.
+Qed.
+Lemma unop_type_of_sound op τ σ :
+  unop_type_of op τ = Some σ → unop_typed op τ σ.
+Proof.
+  destruct τ; intros; simplify_option_equality; constructor.
+  auto using base_unop_type_of_sound.
+Qed.
+Lemma unop_type_of_complete op τ σ :
+  unop_typed op τ σ → unop_type_of op τ = Some σ.
+Proof.
+  destruct 1; simplify_option_equality.
+  by erewrite base_unop_type_of_complete by eauto.
+Qed.
+Lemma binop_type_of_sound op τ1 τ2 σ :
+  binop_type_of op τ1 τ2 = Some σ → binop_typed op τ1 τ2 σ.
+Proof.
+  destruct τ1, τ2; intros; simplify_option_equality; constructor.
+  by apply base_binop_type_of_sound.
+Qed.
+Lemma binop_type_of_complete op τ1 τ2 σ :
+  binop_typed op τ1 τ2 σ → binop_type_of op τ1 τ2 = Some σ.
+Proof.
+  destruct 1; simplify_option_equality.
+  by erewrite base_binop_type_of_complete by eauto.
+Qed.
+Global Instance cast_typed_dec Γ τ σ : Decision (cast_typed Γ τ σ).
+Proof.
+ refine 
+  match decide (τ = σ) with
+  | left _ => left _
+  | right Hτσ =>
+    match τ, σ return τ ≠ σ → Decision (cast_typed Γ τ σ) with
+    | baseT τb, baseT σb => λ _, cast_if (decide (base_cast_typed Γ τb σb))
+    | _, baseT σb => λ _, cast_if (decide (σb = voidT%BT))
+    | _, _ => λ _, right _
+    end Hτσ
+  end; abstract first
+   [ by subst; constructor
+   | by inversion 1; subst;
+      repeat match goal with
+      | H : ¬base_cast_typed _ _ _ |- _ => destruct H; constructor
+      end].
+Defined.
+Lemma cast_typed_weaken Γ1 Γ2 τ σ :
+  cast_typed Γ1 τ σ → Γ1 ⊆ Γ2 → cast_typed Γ2 τ σ.
+Proof. destruct 1; constructor; eauto using base_cast_typed_weaken. Qed.
+Lemma val_unop_ok_weaken Γm1 Γm2 op v :
+  val_unop_ok Γm1 op v → (∀ o, index_alive Γm1 o → index_alive Γm2 o) →
+  val_unop_ok Γm2 op v.
+Proof. unfold val_unop_ok; destruct v; eauto using base_val_unop_ok_weaken. Qed.
+Lemma val_unop_typed Γ Γm op v τ σ :
+  (Γ,Γm) ⊢ v : τ → unop_typed op τ σ → val_unop_ok Γm op v →
+  (Γ,Γm) ⊢ val_unop op v : σ.
+Proof.
+  intros Hvτ Hσ Hop. destruct Hσ; inversion Hvτ; simpl; simplify_equality;
+    done || constructor; eauto using base_val_unop_typed.
+Qed.
+Lemma val_binop_ok_weaken Γ1 Γ2 Γm1 Γm2 op v1 v2 τ1 τ2 :
+  ✓ Γ1 → (Γ1,Γm1) ⊢ v1 : τ1 → (Γ1,Γm1) ⊢ v2 : τ2 → val_binop_ok Γ1 Γm1 op v1 v2 →
+  Γ1 ⊆ Γ2 → (∀ o, index_alive Γm1 o → index_alive Γm2 o) →
+  val_binop_ok Γ2 Γm2 op v1 v2.
+Proof.
+  destruct 2, 1, op; simpl; try done; eauto 2 using base_val_binop_ok_weaken.
+Qed.
+Lemma val_binop_weaken Γ1 Γ2 Γm1 op v1 v2 τ1 τ2 :
+  ✓ Γ1 → (Γ1,Γm1) ⊢ v1 : τ1 → (Γ1,Γm1) ⊢ v2 : τ2 → Γ1 ⊆ Γ2 →
+  val_binop Γ1 op v1 v2 = val_binop Γ2 op v1 v2.
+Proof.
+  destruct 2, 1, op; intros; f_equal'; eauto 2 using base_val_binop_weaken.
+Qed.
+Lemma val_binop_typed Γ Γm op v1 v2 τ1 τ2 σ :
+  ✓ Γ → (Γ,Γm) ⊢ v1 : τ1 → (Γ,Γm) ⊢ v2 : τ2 →
+  binop_typed op τ1 τ2 σ → val_binop_ok Γ Γm op v1 v2 →
+  (Γ,Γm) ⊢ val_binop Γ op v1 v2 : σ.
+Proof.
+  intros ? Hv1τ Hv2τ Hσ Hop.
+  destruct Hσ; inversion Hv1τ; inversion Hv2τ; simplify_equality';
+    done || constructor; eauto using base_val_binop_typed.
+Qed.
+Lemma val_cast_ok_weaken Γ1 Γ2 Γm1 Γm2 v τ σ :
+  ✓ Γ1 → (Γ1,Γm1) ⊢ v : τ → val_cast_ok Γ1 Γm1 σ v → Γ1 ⊆ Γ2 →
+  (∀ o, index_alive Γm1 o → index_alive Γm2 o) → val_cast_ok Γ2 Γm2 σ v.
+Proof. destruct 2, σ; simpl; eauto using base_val_cast_ok_weaken. Qed.
+Lemma val_cast_typed Γ Γm v τ σ :
+  ✓ Γ → (Γ,Γm) ⊢ v : τ → cast_typed Γ τ σ → val_cast_ok Γ Γm σ v →
+  (Γ,Γm) ⊢ val_cast σ v : σ.
+Proof.
+  intros ? Hvτ Hσ Hok. destruct Hσ; inversion Hvτ; simplify_equality';
+    repeat typed_constructor;
+    eauto using base_val_cast_typed, TVoid_cast_typed, base_cast_typed_self.
+Qed.
+
+Lemma val_true_refine Γ f Γm1 Γm2 v1 v2 τ :
+  v1 ⊑{Γ,f@Γm1↦Γm2} v2 : τ → val_true Γm1 v1 → val_true Γm2 v2.
+Proof. destruct 1; simpl; eauto using base_val_true_refine. Qed.
+Lemma val_false_refine Γ f Γm1 Γm2 v1 v2 τ :
+  v1 ⊑{Γ,f@Γm1↦Γm2} v2 : τ → val_false v1 → val_false v2.
+Proof. destruct 1; simpl; eauto using base_val_false_refine. Qed.
+Lemma val_true_false_refine Γ f Γm1 Γm2 v1 v2 τ :
+  val_true Γm1 v1 → val_false v2 → v1 ⊑{Γ,f@Γm1↦Γm2} v2 : τ → False.
+Proof.
+  intros. by destruct (val_true_false_dec Γm2 v2)
+    as [[[??]|[??]]|[??]]; eauto using val_true_refine.
+Qed.
+Lemma val_false_true_refine Γ f Γm1 Γm2 v1 v2 τ :
+  val_false v1 → val_true Γm2 v2 → v1 ⊑{Γ,f@Γm1↦Γm2} v2 : τ → False.
+Proof.
+  intros. by destruct (val_true_false_dec Γm2 v2)
+    as [[[??]|[??]]|[??]]; eauto using val_false_refine.
+Qed.
+Lemma val_true_refine_inv Γ f Γm1 Γm2 v1 v2 τ :
+  v1 ⊑{Γ,f@Γm1↦Γm2} v2 : τ → val_true Γm2 v2 →
+  val_true Γm1 v1 ∨ ¬val_true Γm1 v1 ∧ ¬val_false v1.
+Proof.
+  intros. destruct (val_true_false_dec Γm1 v1)
+    as [[[??]|[??]]|[??]]; eauto using val_false_true_refine.
+Qed.
+Lemma val_false_refine_inv Γ f Γm1 Γm2 v1 v2 τ :
+  v1 ⊑{Γ,f@Γm1↦Γm2} v2 : τ → val_false v2 →
+  val_false v1 ∨ ¬val_true Γm1 v1 ∧ ¬val_false v1.
+Proof.
+  intros. destruct (val_true_false_dec Γm1 v1)
+    as [[[??]|[??]]|[??]]; eauto using val_true_false_refine.
+Qed.
+Lemma val_unop_ok_refine Γ f Γm1 Γm2 op v1 v2 τ :
+  v1 ⊑{Γ,f@Γm1↦Γm2} v2 : τ → val_unop_ok Γm1 op v1 → val_unop_ok Γm2 op v2.
+Proof. destruct op, 1; simpl; eauto using base_val_unop_ok_refine. Qed.
+Lemma val_unop_refine Γ f Γm1 Γm2 op v1 v2 τ σ :
+  ✓ Γ → unop_typed op τ σ → val_unop_ok Γm1 op v1 →
+  v1 ⊑{Γ,f@Γm1↦Γm2} v2 : τ → val_unop op v1 ⊑{Γ,f@Γm1↦Γm2} val_unop op v2 : σ.
+Proof.
+  destruct 2; inversion 2; intros; simplify_equality';
+    refine_constructor; eauto using base_val_unop_refine.
+Qed.
+Lemma val_binop_ok_refine Γ f Γm1 Γm2 op v1 v2 v3 v4 τ1 τ3 σ :
+  ✓ Γ → binop_typed op τ1 τ3 σ →
+  v1 ⊑{Γ,f@Γm1↦Γm2} v2 : τ1 → v3 ⊑{Γ,f@Γm1↦Γm2} v4 : τ3 →
+  val_binop_ok Γ Γm1 op v1 v3 → val_binop_ok Γ Γm2 op v2 v4.
+Proof.
+  unfold val_binop_ok; destruct 2; do 2 inversion 1;
+    simplify_equality'; eauto using base_val_binop_ok_refine.
+Qed.
+Lemma val_binop_refine Γ f Γm1 Γm2 op v1 v2 v3 v4 τ1 τ3 σ :
+  ✓ Γ → binop_typed op τ1 τ3 σ → val_binop_ok Γ Γm1 op v1 v3 →
+  v1 ⊑{Γ,f@Γm1↦Γm2} v2 : τ1 → v3 ⊑{Γ,f@Γm1↦Γm2} v4 : τ3 →
+  val_binop Γ op v1 v3 ⊑{Γ,f@Γm1↦Γm2} val_binop Γ op v2 v4 : σ.
+Proof.
+  destruct 2; intro; do 2 inversion 1; simplify_equality';
+    refine_constructor; eauto using base_val_binop_refine.
+Qed.
+Lemma val_cast_ok_refine Γ Γm1 Γm2 f v1 v2 τ σ :
+  ✓ Γ → v1 ⊑{Γ,f@Γm1↦Γm2} v2 : τ →
+  val_cast_ok Γ Γm1 σ v1 → val_cast_ok Γ Γm2 σ v2.
+Proof.
+  unfold val_cast_ok; destruct σ, 2; eauto using base_val_cast_ok_refine.
+Qed.
+Lemma val_cast_refine Γ f Γm1 Γm2 v1 v2 τ σ :
+  ✓ Γ → cast_typed Γ τ σ → val_cast_ok Γ Γm1 σ v1 →
+  v1 ⊑{Γ,f@Γm1↦Γm2} v2 : τ → val_cast σ v1 ⊑{Γ,f@Γm1↦Γm2} val_cast σ v2 : σ.
+Proof.
+  destruct 2; inversion 2; simplify_equality; repeat refine_constructor;
+    eauto using base_val_cast_refine, TVoid_cast_typed, base_cast_typed_self.
+Qed.
+End properties.
