type_system.v
@@ -1,6 +1,6 @@
 (* Copyright (c) 2012-2014, Robbert Krebbers. *)
 (* This file is distributed under the terms of the BSD license. *)
-Require Export state.
+Require Export operations state.
 Local Open Scope expr_scope.
 Local Open Scope ctype_scope.
 
